rt riscv refine: finish Retype_R.thy
Signed-off-by: Michael McInerney <m.mcinerney@unsw.edu.au>

proof/refine/RISCV64/Retype_R.thy
@@ -78,7 +78,7 @@ definition makeObjectKO
   "makeObjectKO dev us d ty \<equiv> case ty of
       Inl KOUserData \<Rightarrow> Some KOUserData
     | Inl (KOArch (KOASIDPool _)) \<Rightarrow> Some (KOArch (KOASIDPool makeObject))
-    | Inr (APIObjectType ArchTypes_H.TCBObject) \<Rightarrow> Some (KOTCB makeObject)
+    | Inr (APIObjectType ArchTypes_H.TCBObject) \<Rightarrow> Some (KOTCB (tcbDomain_update (\<lambda>_. d) makeObject))
     | Inr (APIObjectType ArchTypes_H.EndpointObject) \<Rightarrow> Some (KOEndpoint makeObject)
     | Inr (APIObjectType ArchTypes_H.NotificationObject) \<Rightarrow> Some (KONotification makeObject)
     | Inr (APIObjectType ArchTypes_H.CapTableObject) \<Rightarrow> Some (KOCTE makeObject)
@@ -107,6 +107,12 @@ lemma valid_obj_makeObject_tcb [simp]:
   unfolding valid_obj'_def valid_tcb'_def  valid_tcb_state'_def
   by (clarsimp simp: makeObject_tcb makeObject_cte tcb_cte_cases_def minBound_word cteSizeBits_def)
 
+lemma valid_obj_makeObject_tcb_tcbDomain_update [simp]:
+  "d \<le> maxDomain \<Longrightarrow> valid_obj' (KOTCB (tcbDomain_update (\<lambda>_. d) makeObject)) s"
+  unfolding valid_obj'_def valid_tcb'_def  valid_tcb_state'_def
+  by (clarsimp simp: makeObject_tcb makeObject_cte objBits_simps'
+                     tcb_cte_cases_def maxDomain_def maxPriority_def numPriorities_def minBound_word)
+
 lemma valid_obj_makeObject_endpoint [simp]:
   "valid_obj' (KOEndpoint makeObject) s"
   unfolding valid_obj'_def valid_ep'_def
@@ -116,6 +122,31 @@ lemma valid_obj_makeObject_notification [simp]:
   "valid_obj' (KONotification makeObject) s"
   unfolding valid_obj'_def valid_ntfn'_def
   by (clarsimp simp: makeObject_notification)
+
+lemma valid_obj_makeObject_reply [simp]:
+  "valid_obj' (KOReply makeObject) s"
+  unfolding valid_obj'_def valid_reply'_def
+  by (clarsimp simp: makeObject_reply)
+
+lemma valid_sc_size'_makeObject_sc':
+  "sc_size_bounds us \<Longrightarrow>
+     valid_sched_context_size'
+       (scRefills_update (\<lambda>_. replicate (refillAbsoluteMax' us) emptyRefill) makeObject)"
+  by (clarsimp simp: makeObject_sc valid_sched_context_size'_def scBits_simps
+                     objBits_def objBitsKO_def)
+
+lemma MIN_REFILLS_refillAbsoluteMax'[simp]:
+  "minSchedContextBits \<le> us \<Longrightarrow> MIN_REFILLS \<le> refillAbsoluteMax' us"
+  using MIN_REFILLS_le_minRefillLength order.trans refillAbsoluteMax'_lb by auto
+
+lemma valid_obj_makeObject_sched_context [simp]:
+  "sc_size_bounds us \<Longrightarrow>
+     valid_obj' (KOSchedContext (scRefills_update
+                   (\<lambda>_. replicate (refillAbsoluteMax' us) emptyRefill) makeObject)) s"
+  unfolding valid_obj'_def valid_sched_context'_def
+  using refillAbsoluteMax'_lb sc_size_bounds_def minRefillLength_ARM
+  by (clarsimp simp: valid_sc_size'_makeObject_sc')
+     (clarsimp simp: makeObject_sc scBits_inverse_us)
 
 lemma valid_obj_makeObject_user_data [simp]:
   "valid_obj' (KOUserData) s"
@@ -428,7 +459,7 @@ lemma makeObjectKO_eq:
   "(v = KOCTE cte) =
        (tp = Inr (APIObjectType ArchTypes_H.CapTableObject) \<and> cte = makeObject)"
   "(v = KOTCB tcb) =
-       (tp = Inr (APIObjectType ArchTypes_H.TCBObject) \<and> tcb = makeObject)"
+       (tp = Inr (APIObjectType ArchTypes_H.TCBObject) \<and> tcb = (tcbDomain_update (\<lambda>_. d) makeObject))"
   using x
   by (simp add: makeObjectKO_def eq_commute
          split: apiobject_type.split_asm sum.split_asm kernel_object.split_asm
@@ -487,9 +518,9 @@ lemma cte_wp_at_retype':
       and pv: "pspace_aligned' s" "pspace_distinct' s"
      and pv': "pspace_aligned' (ksPSpace_update (\<lambda>x xa. if xa \<in> set addrs then Some obj else ksPSpace s xa) s)"
               "pspace_distinct' (ksPSpace_update (\<lambda>x xa. if xa \<in> set addrs then Some obj else ksPSpace s xa) s)"
-      and al: "\<forall>x \<in> set addrs. is_aligned x (objBitsKO obj)" "objBitsKO obj < word_bits"
+      and al: "\<forall>x \<in> set addrs. is_aligned x (objBitsKO obj)""objBitsKO obj < word_bits"
       and pn: "\<forall>x \<in> set addrs. ksPSpace s x = None"
-  shows
+   shows
   "cte_wp_at' P p (ksPSpace_update (\<lambda>x xa. if xa \<in> set addrs then Some obj else ksPSpace s xa) s)
       = (if tp = Inr (APIObjectType ArchTypes_H.CapTableObject) \<and> p \<in> set addrs
            \<or> tp = Inr (APIObjectType ArchTypes_H.TCBObject)
@@ -502,23 +533,24 @@ lemma cte_wp_at_retype':
     apply (subgoal_tac "(\<exists>P :: cte \<Rightarrow> bool. obj_at' P p ?s')
                           \<longrightarrow> (\<not> (\<exists>P :: tcb \<Rightarrow> bool. obj_at' P (p && ~~ mask tcbBlockSizeBits) ?s'))")
      apply (simp only: cte_wp_at_obj_cases_mask foldr_update_obj_at'[OF pv pv' al])
-     apply (simp add: the_ctes_makeObject makeObjectKO_eq [OF ko] makeObject_cte dom_def
-                 split del: if_split
-                 cong: if_cong)
+     apply (simp    add: projectKOs the_ctes_makeObject
+                         makeObjectKO_eq [OF ko]
+                         makeObject_cte
+              split del: if_split
+                   cong: if_cong)
      apply (insert al ko)
-     apply (simp, safe, simp_all)
-      apply fastforce
-     apply fastforce
-    apply (clarsimp elim!: obj_atE' simp: objBits_simps)
+     apply simp
+     apply (safe; simp)
+              apply ((fastforce simp: makeObjectKO_def makeObject_cte makeObject_tcb tcb_cte_cases_def
+                              split: if_split_asm)+)[10]
+    apply (clarsimp elim!: obj_atE' simp: projectKOs objBits_simps)
     apply (drule ps_clearD[where y=p and n=tcbBlockSizeBits])
        apply simp
       apply (rule order_trans_rules(17))
        apply (clarsimp cong: if_cong)
       apply (rule word_and_le2)
-     apply (simp add: word_neg_and_le[simplified field_simps])
-    apply simp
-   apply (clarsimp elim!: obj_atE' simp: pn)
-  apply (clarsimp elim!: obj_atE' simp: pn)
+     apply (rule word_neg_and_le[simplified field_simps])
+    apply (clarsimp elim!: obj_atE' simp: pn)+
   done
 
 lemma ctes_of_retype:
@@ -582,11 +614,12 @@ lemma null_filter_ctes_retype:
    apply (insert ko[symmetric], simp add: makeObjectKO_def objBits_simps)
    apply clarsimp
    apply (subst(asm) subtract_mask[symmetric],
-          erule_tac v="if x \<in> set addrs then KOTCB makeObject else KOCTE cte"
+          erule_tac v="if x \<in> set addrs then KOTCB (tcbDomain_update (\<lambda>_. d) makeObject)
+                                        else KOCTE cte"
                 in tcb_space_clear)
        apply (simp add: is_aligned_mask word_bw_assocs)
       apply assumption
-     apply simp
+     apply fastforce
     apply simp
    apply (simp add: pn)
   apply (clarsimp simp: makeObjectKO_def)
@@ -1041,10 +1074,13 @@ qed
 
 lemma retype_aligned_distinct':
   assumes vs': "pspace_aligned' s'" "pspace_distinct' s'"
+      and bd : "pspace_bounded' s'"
       and pn': "pspace_no_overlap' ptr sz s'"
       and cover: "range_cover ptr sz (objBitsKO ko) n "
   shows
   "pspace_distinct' (s' \<lparr>ksPSpace := foldr (\<lambda>addr. data_map_insert addr ko)
+                                             (new_cap_addrs n ptr ko) (ksPSpace s')\<rparr>)"
+  "pspace_bounded' (s' \<lparr>ksPSpace := foldr (\<lambda>addr. data_map_insert addr ko)
                                              (new_cap_addrs n ptr ko) (ksPSpace s')\<rparr>)"
   "pspace_aligned' (s' \<lparr>ksPSpace := foldr (\<lambda>addr. data_map_insert addr ko)
                                              (new_cap_addrs n ptr ko) (ksPSpace s')\<rparr>)"
@@ -1103,6 +1139,15 @@ proof -
     apply (drule pspace_no_overlapD' [OF _ pn'])
     apply (simp add: mask_def add_diff_eq)
     done
+
+  show bd': "pspace_bounded' ?s'" using bd
+    apply (subst foldr_upd_app_if[folded data_map_insert_def])
+    apply (clarsimp simp: pspace_bounded'_def split: if_split_asm)
+    using cover
+     apply (simp add: range_cover_def word_bits_def)
+    apply (drule bspec, erule domI, simp)
+    done
+
 qed
 
 definition
@@ -1257,6 +1302,7 @@ proof -
     using sr pr
     unfolding sc_replies_relation_def
     apply (clarsimp simp: sc_replies_of_scs_def map_project_def scs_of_kh_def
+                   elim!: opt_mapE
                    split: Structures_A.kernel_object.split_asm)
     apply (rename_tac sc n'; drule_tac x=p and y="sc_replies sc" in spec2)
     apply (clarsimp simp: foldr_upd_app_if[folded data_map_insert_def] split: if_split_asm)
@@ -1325,7 +1371,7 @@ lemma retype_state_relation:
   let ?tp = "APIType_map2 ty"
   let ?al = "retype_addrs ptr ?tp n us"
 
-  note pad' = retype_aligned_distinct' [OF vs' pn' cover']
+  note pad' = retype_aligned_distinct' [OF vs' bd' pn' cover']
   thus pa': "pspace_aligned' (s'\<lparr>ksPSpace := ?ps'\<rparr>)"
    and pd': "pspace_distinct' (s'\<lparr>ksPSpace := ?ps'\<rparr>)"
     by simp_all
@@ -1546,7 +1592,7 @@ lemma objBitsKO_gt_0: "0 < objBitsKO ko"
     apply (simp_all add:archObjSize_def bit_simps)
   done
 
-lemma kheap_ekheap_double_gets: "(\<And>rv erv rv'. pspace_relation rv rv' \<Longrightarrow> ekheap_relation erv rv' \<Longrightarrow> corres r (R rv erv) (R' rv') (b rv erv) (d rv')) \<Longrightarrow>
+\<comment> \<open>lemma kheap_ekheap_double_gets: "(\<And>rv erv rv'. pspace_relation rv rv' \<Longrightarrow> ekheap_relation erv rv' \<Longrightarrow> corres r (R rv erv) (R' rv') (b rv erv) (d rv')) \<Longrightarrow>
 corres r (\<lambda>s. R (kheap s) (ekheap s) s) (\<lambda>s. R' (ksPSpace s) s) (do x \<leftarrow> gets kheap; xa \<leftarrow> gets ekheap; b x xa od) (gets ksPSpace >>= d)"
   apply (rule corres_symb_exec_l)
      apply (rule corres_guard_imp)
@@ -1738,26 +1784,27 @@ apply (clarsimp simp: retype_region_def retype_region2_def when_def bind_assoc)
 apply (subst retype_region_ext_modify_kheap_futz'[simplified bind_assoc])
 apply (subst retype_region2_ext_retype_region_ext_futz[symmetric])
 apply (simp add: bind_assoc)
-done
+done\<close>
 
 lemma getObject_tcb_gets:
   "getObject addr >>= (\<lambda>x::tcb. gets proj >>= (\<lambda>y. G x y))
- = gets proj >>= (\<lambda>y. getObject addr >>= (\<lambda>x. G x y))"
-by (auto simp: exec_gets fun_eq_iff intro: bind_apply_cong dest!: in_inv_by_hoareD[OF getObject_inv_tcb])
+   = gets proj >>= (\<lambda>y. getObject addr >>= (\<lambda>x. G x y))"
+  by (auto simp: exec_gets fun_eq_iff intro: bind_apply_cong
+           dest!: in_inv_by_hoareD[OF getObject_tcb_inv])
 
 lemma setObject_tcb_gets_ksCurDomain:
   "setObject addr (tcb::tcb) >>= (\<lambda>_. gets ksCurDomain >>= G)
- = gets ksCurDomain >>= (\<lambda>x. setObject addr tcb >>= (\<lambda>_. G x))"
-apply (clarsimp simp: exec_gets fun_eq_iff)
-apply (rule bind_apply_cong)
- apply simp
-apply (drule_tac P1="\<lambda>cdom. cdom = ksCurDomain x" in use_valid[OF _ setObject_cd_inv])
-apply (simp_all add: exec_gets)
-done
+   = gets ksCurDomain >>= (\<lambda>x. setObject addr tcb >>= (\<lambda>_. G x))"
+  apply (clarsimp simp: exec_gets fun_eq_iff)
+  apply (rule bind_apply_cong)
+   apply simp
+  apply (drule_tac P1="\<lambda>cdom. cdom = ksCurDomain x" in use_valid[OF _ setObject_cd_inv])
+   apply (simp_all add: exec_gets)
+  done
 
 lemma curDomain_mapM_x_futz:
   "curDomain >>= (\<lambda>cdom. mapM_x (threadSet (F cdom)) addrs)
- = mapM_x (\<lambda>addr. curDomain >>= (\<lambda>cdom. threadSet (F cdom) addr)) addrs"
+   = mapM_x (\<lambda>addr. curDomain >>= (\<lambda>cdom. threadSet (F cdom) addr)) addrs"
 proof(induct addrs)
   case Nil thus ?case
     by (simp add: curDomain_def mapM_x_def sequence_x_def bind_def gets_def get_def return_def)
@@ -1788,31 +1835,26 @@ The existing proof continues below.
 
 *)
 
-lemma modify_ekheap_update_ekheap:
-  "modify (\<lambda>s. ekheap_update f s) = do s \<leftarrow> gets ekheap; modify (\<lambda>s'. s'\<lparr>ekheap := f s\<rparr>) od"
-by (simp add: modify_def gets_def get_def put_def bind_def return_def split_def fun_eq_iff)
-
 lemma corres_retype':
   assumes    not_zero: "n \<noteq> 0"
   and         aligned: "is_aligned ptr (objBitsKO ko + gbits)"
-  and    obj_bits_api: "obj_bits_api (APIType_map2 ty) us =
-                        objBitsKO ko + gbits"
-  and           check: "(sz < obj_bits_api (APIType_map2 ty)  us)
-                           = (sz < objBitsKO ko + gbits)"
-  and             usv: "APIType_map2 ty = Structures_A.CapTableObject \<Longrightarrow> 0 < us"
-  and              ko: "makeObjectKO dev ty = Some ko"
+  and    obj_bits_api: "obj_bits_api (APIType_map2 ty) us = objBitsKO ko + gbits"
+  and           check: "(sz < obj_bits_api (APIType_map2 ty)  us) = (sz < objBitsKO ko + gbits)"
+  and              ko: "makeObjectKO dev us d ty = Some ko"
+  and            tysc: "ty = Inr (APIObjectType SchedContextObject) \<longrightarrow> min_sched_context_bits \<le> us"
   and             orr: "obj_bits_api (APIType_map2 ty) us \<le> sz \<Longrightarrow>
-                        obj_relation_retype
-                          (default_object (APIType_map2 ty) dev us) ko"
+                        obj_relation_retype (default_object (APIType_map2 ty) dev us d) ko"
   and           cover: "range_cover ptr sz (obj_bits_api (APIType_map2 ty) us) n"
   shows "corres (\<lambda>rv rv'. rv' = g rv)
-  (\<lambda>s. valid_pspace s \<and> pspace_no_overlap_range_cover ptr sz s
-     \<and> valid_mdb s \<and> valid_etcbs s \<and> valid_list s)
-  (\<lambda>s. pspace_aligned' s \<and> pspace_distinct' s \<and> pspace_no_overlap' ptr sz s)
-  (retype_region2 ptr n us (APIType_map2 ty) dev)
-  (do addrs \<leftarrow> createObjects ptr n ko gbits;
-      _ \<leftarrow> modify (update_gs (APIType_map2 ty) us (set addrs));
-      return (g addrs) od)"
+                (\<lambda>s. valid_pspace s \<and> pspace_no_overlap_range_cover ptr sz s
+                     \<and> valid_mdb s \<and> valid_list s)
+                (\<lambda>s. pspace_aligned' s \<and> pspace_distinct' s \<and> pspace_no_overlap' ptr sz s
+                      \<and> (ty = Inr (APIObjectType TCBObject) \<longrightarrow> d = ksCurDomain s))
+                (retype_region ptr n us (APIType_map2 ty) dev)
+                (do addrs \<leftarrow> createObjects ptr n ko gbits;
+                    _ \<leftarrow> modify (update_gs (APIType_map2 ty) us (set addrs));
+                    return (g addrs)
+                 od)"
   (is "corres ?r ?P ?P' ?C ?A")
 proof -
   note data_map_insert_def[simp del]
@@ -1892,7 +1934,7 @@ proof -
      by (simp add: obj_bits_api ko)
   show ?thesis
   including no_take_bit
-  apply (simp add: when_def retype_region2_def createObjects'_def
+  apply (simp add: when_def retype_region_def createObjects'_def
                    createObjects_def aligned obj_bits_api[symmetric]
                    ko[symmetric] al' shiftl_t2n data_map_insert_def[symmetric]
                    is_aligned_mask[symmetric] split_def unless_def
@@ -1900,80 +1942,92 @@ proof -
         split del: if_split)
   apply (subst retype_addrs_fold)+
   apply (subst if_P)
-   using ko
-   apply (clarsimp simp: makeObjectKO_def)
-  apply (simp add: bind_assoc retype_region2_ext_def)
-  apply (rule corres_guard_imp)
-    apply (subst modify_ekheap_update_ekheap)
-    apply (simp only: bind_assoc)
-    apply (rule kheap_ekheap_double_gets)
-    apply (rule corres_symb_exec_r)
-       apply (simp add: not_less modify_modify bind_assoc[symmetric]
-                          obj_bits_api[symmetric] shiftl_t2n upto_enum_red'
+    using ko
+    apply (clarsimp simp: makeObjectKO_def)
+   apply (simp add: bind_assoc)
+   apply (rule corres_guard_imp)
+     apply (rule_tac r'=pspace_relation in corres_split')
+        apply (clarsimp dest!: state_relation_pspace_relation)
+       apply (simp add: gets_def)
+       apply (rule corres_symb_exec_l[rotated])
+          apply (rule exs_valid_get)
+         apply (rule get_sp)
+        apply (simp add: get_def no_fail_def)
+       apply (rule corres_symb_exec_r)
+          apply (simp add: not_less modify_modify bind_assoc[symmetric]
+                           obj_bits_api[symmetric] shiftl_t2n upto_enum_red'
                            range_cover.unat_of_nat_n[OF cover])
-       apply (rule corres_split_nor[OF corres_trivial])
+          apply (rule corres_guard_imp)
+            apply (rule corres_split_nor[OF corres_trivial])
           apply (clarsimp simp: retype_addrs_fold[symmetric] ptr_add_def upto_enum_red' not_zero'
                                 range_cover.unat_of_nat_n[OF cover] word_le_sub1
                           simp del: word_of_nat_eq_0_iff)
-         apply (rule_tac f=g in arg_cong)
-         apply clarsimp
-         apply (rename_tac x eps ps)
-         apply (rule_tac P="\<lambda>s. x = kheap s \<and> eps = ekheap (s) \<and> ?P s" and
-                         P'="\<lambda>s. ps = ksPSpace s \<and> ?P' s" in corres_modify)
-         apply (simp add: set_retype_addrs_fold new_caps_adds_fold)
-         apply (erule retype_state_relation[OF _ _ _ _ _ _ _ _ _ cover _ _ orr],
-                simp_all add: ko not_zero obj_bits_api
-                              bound[simplified obj_bits_api ko])[1]
-        apply wp+
-      apply (clarsimp split: option.splits)
-      apply (intro conjI impI)
-       apply (clarsimp|wp)+
-     apply (clarsimp split: option.splits)
-     apply wpsimp
-    apply (clarsimp split: option.splits)
-    apply (intro conjI impI)
-     apply wp
-    apply (clarsimp simp:lookupAround2_char1)
-    apply wp
-    apply (clarsimp simp: obj_bits_api ko)
-    apply (drule(1) pspace_no_overlap_disjoint')
-    apply (rule_tac x1 = a in ccontr[OF in_empty_interE])
-      apply simp
-     apply (clarsimp simp: not_less shiftL_nat)
-     apply (erule order_trans)
-     apply (subst p_assoc_help)
-     apply (subst word_plus_and_or_coroll2[symmetric,where w = "mask sz"])
-     apply (subst add.commute)
-     apply (subst add.assoc)
-     apply (rule word_plus_mono_right)
-      using cover
-      apply -
-      apply (rule iffD2[OF word_le_nat_alt])
-      apply (subst word_of_nat_minus)
-       using not_zero
-       apply simp
-      apply (rule le_trans[OF unat_plus_gt])
-      apply simp
-      apply (subst unat_minus_one)
-       apply (subst mult.commute)
-       apply (rule word_power_nonzero_64)
-         apply (rule of_nat_less_pow_64[OF n_estimate])
-         apply (simp add:word_bits_def objBitsKO_gt_0 ko)
-        apply (simp add:range_cover_def obj_bits_api ko word_bits_def)
-       apply (cut_tac not_zero',clarsimp simp:ko)
-      apply(clarsimp simp:field_simps ko)
-      apply (subst unat_sub[OF word_1_le_power])
-       apply (simp add:range_cover_def)
-      apply (subst diff_add_assoc[symmetric])
-       apply (cut_tac unat_of_nat_n',simp add:ko)
-      apply (clarsimp simp: obj_bits_api ko)
-      apply (rule diff_le_mono)
-      apply (frule range_cover.range_cover_compare_bound)
-      apply (cut_tac obj_bits_api unat_of_nat_shift')
-      apply (clarsimp simp:add.commute range_cover_def ko)
-     apply (rule is_aligned_no_wrap'[OF is_aligned_neg_mask,OF le_refl ])
-     apply (simp add:range_cover_def domI)+
-  done
+               apply (rule_tac f=g in arg_cong)
+               apply clarsimp
+              apply (rename_tac ps ps' sa)
+              apply (rule_tac P="\<lambda>s. ps = kheap s \<and> sa = s \<and> ?P s" and
+                              P'="\<lambda>s. ps' = ksPSpace s \<and> ?P' s" in corres_modify)
+              apply(frule curdomain_relation[THEN sym])
+              apply (simp add: set_retype_addrs_fold new_caps_adds_fold)
+              apply (drule retype_state_relation[OF _ _ _ _ _ _ _ _ _ tysc cover _ _ orr],
+                     simp_all add: ko not_zero obj_bits_api
+                                   bound[simplified obj_bits_api ko])[1]
+                apply (erule pspace_relation_pspace_bounded')
+               apply (cases ty; simp; rename_tac tp; case_tac tp;
+                      clarsimp simp: default_object_def APIType_map2_def
+                              split: arch_kernel_object.splits apiobject_type.splits)
+             apply wpsimp+
+           apply simp+
+         apply (clarsimp split: option.splits)
+         apply (intro conjI impI)
+          apply (clarsimp|wp)+
+        apply (clarsimp split: option.splits)
+        apply wpsimp
+       apply (clarsimp split: option.splits)
+       apply (intro conjI impI)
+        apply wp
+       apply (clarsimp simp:lookupAround2_char1)
+       apply wp
+       apply (clarsimp simp: obj_bits_api ko)
+       apply (drule(1) pspace_no_overlap_disjoint')
+       apply (rule_tac x1 = a in ccontr[OF in_empty_interE])
+         apply simp
+        apply (clarsimp simp: not_less shiftL_nat)
+        apply (erule order_trans)
+        apply (subst p_assoc_help)
+        apply (subst word_plus_and_or_coroll2[symmetric,where w = "mask sz"])
+        apply (subst add.commute)
+        apply (subst add.assoc)
+        apply (rule word_plus_mono_right)
+         using cover
+         apply -
+         apply (rule iffD2[OF word_le_nat_alt])
+         apply (subst word_of_nat_minus)
+          using not_zero
+          apply simp
+         apply (rule le_trans[OF unat_plus_gt])
+         apply simp
+         apply (subst unat_minus_one)
+          apply (subst mult.commute)
+          apply (rule word_power_nonzero_64)
+            apply (rule of_nat_less_pow_64[OF n_estimate])
+            apply (simp add:word_bits_def objBitsKO_gt_0 ko)
+           apply (simp add:range_cover_def obj_bits_api ko word_bits_def)
+          apply (cut_tac not_zero',clarsimp simp:ko)
+         apply(clarsimp simp:field_simps ko)
+         apply (subst unat_sub[OF word_1_le_power])
+          apply (simp add:range_cover_def)
+         apply (subst diff_add_assoc[symmetric])
+          apply (cut_tac unat_of_nat_n',simp add:ko)
+         apply (clarsimp simp: obj_bits_api ko)
+         apply (rule diff_le_mono)
+         apply (frule range_cover.range_cover_compare_bound)
+         apply (cut_tac obj_bits_api unat_of_nat_shift')
+         apply (clarsimp simp:add.commute range_cover_def ko)
+        apply (rule is_aligned_no_wrap'[OF is_aligned_neg_mask,OF le_refl ])
+        apply (simp add:range_cover_def domI)+
+      apply wpsimp+
+   done
 qed
 
 lemma createObjects_corres':
@@ -1997,6 +2051,7 @@ lemmas retype_aligned_distinct'' = retype_aligned_distinct'
 
 lemma retype_ko_wp_at':
   assumes vs: "pspace_aligned' s" "pspace_distinct' s"
+     and  bd:  "pspace_bounded' s"
      and  pn: "pspace_no_overlap' ptr sz s"
    and cover: "range_cover ptr sz (objBitsKO obj) n"
   shows
@@ -2006,14 +2061,16 @@ lemma retype_ko_wp_at':
                          else ko_wp_at' P p s)"
   apply (subst foldr_upd_app_if[folded data_map_insert_def])
   apply (rule foldr_update_ko_wp_at' [OF vs])
-    apply (simp add: retype_aligned_distinct'' [OF vs pn cover])+
-  apply (rule new_cap_addrs_aligned)
+    apply (simp add: retype_aligned_distinct'' [OF vs bd pn cover])+
+   apply (rule new_cap_addrs_aligned)
+   using cover
+   apply (simp add:range_cover_def cover)
   using cover
-  apply (simp add:range_cover_def cover)
+  apply (simp add:range_cover_def word_bits_def)
   done
 
 lemma retype_obj_at':
-  assumes vs: "pspace_aligned' s" "pspace_distinct' s"
+  assumes vs: "pspace_aligned' s" "pspace_distinct' s" "pspace_bounded' s"
      and  pn: "pspace_no_overlap' ptr sz s"
      and cover: "range_cover ptr sz (objBitsKO obj) n"
   shows
@@ -2023,10 +2080,10 @@ lemma retype_obj_at':
                          else obj_at' P p s)"
   unfolding obj_at'_real_def
   apply (rule retype_ko_wp_at'[OF vs pn cover])
-done
+  done
 
 lemma retype_obj_at_disj':
-  assumes vs: "pspace_aligned' s" "pspace_distinct' s"
+  assumes vs: "pspace_aligned' s" "pspace_distinct' s" "pspace_bounded' s"
      and  pn: "pspace_no_overlap' ptr sz s"
      and cover: "range_cover ptr sz (objBitsKO obj) n"
   shows
@@ -2050,8 +2107,8 @@ lemma createObjects_ko_at_strg:
   assumes    cover: "range_cover ptr sz ((objBitsKO ko) + gbits) n"
   assumes    not_0: "n\<noteq> 0"
   assumes       pi: "projectKO_opt ko  = Some val"
-  shows "\<lbrace>\<lambda>s. pspace_no_overlap' ptr sz s \<and> pspace_aligned' s \<and> pspace_distinct' s\<rbrace>
-             createObjects ptr n ko gbits
+  shows "\<lbrace>\<lambda>s. pspace_no_overlap' ptr sz s \<and> pspace_aligned' s \<and> pspace_distinct' s \<and> pspace_bounded' s\<rbrace>
+         createObjects ptr n ko gbits
          \<lbrace>\<lambda>r s. \<forall>x \<in> set r. \<forall>offs < 2 ^ gbits. ko_at' val (x + (offs << objBitsKO ko)) s\<rbrace>"
 proof -
   have shiftr_not_zero:" 1 \<le> ((of_nat n)::machine_word) << gbits"
@@ -2141,24 +2198,19 @@ proof -
   apply unat_arith
   done
   show ?thesis
-  apply (simp add: split_def createObjects_def lookupAround2_pspace_no
-                   alignError_def unless_def createObjects'_def)
-  apply (rule hoare_pre)
-   apply (wp|simp add:data_map_insert_def[symmetric]
-     cong: if_cong del: fun_upd_apply data_map_insert_def)+
-   apply (wpc|wp|clarsimp simp del:fun_upd_apply)+
-   apply (subst new_cap_addrs_fold'[OF shiftr_not_zero])+
-   apply (subst data_map_insert_def[symmetric])+
-   apply (subst retype_obj_at_disj')
-     apply (simp add:valid_pspace'_def unat_of_nat_shiftl)+
-     apply (rule range_cover_rel[OF cover])
-     apply simp+
-   apply (subst retype_obj_at_disj')
-     apply (simp add:valid_pspace'_def unat_of_nat_shiftl)+
-     apply (rule range_cover_rel[OF cover])
-     apply simp+
-  using range_cover.unat_of_nat_n_shift[OF cover,where gbits = gbits,simplified] pi
-  apply (simp add: in_new)
+    apply (simp add: split_def createObjects_def lookupAround2_pspace_no
+                     alignError_def unless_def createObjects'_def)
+    apply (wp|simp add:data_map_insert_def[symmetric]
+                   cong: if_cong del: fun_upd_apply data_map_insert_def)+
+       apply (wpc|wp|clarsimp simp del:fun_upd_apply)+
+    apply (subst new_cap_addrs_fold'[OF shiftr_not_zero])+
+    apply (subst data_map_insert_def[symmetric])+
+    apply (subst retype_obj_at_disj'; simp add:valid_pspace'_def unat_of_nat_shiftl)+
+     apply (rule range_cover_rel[OF cover]; simp)
+    apply (subst retype_obj_at_disj'; simp add:valid_pspace'_def unat_of_nat_shiftl)
+     apply (rule range_cover_rel[OF cover]; simp)
+    using range_cover.unat_of_nat_n_shift[OF cover,where gbits = gbits,simplified] pi
+    apply (simp add: in_new)
   done
 qed
 
@@ -2170,7 +2222,7 @@ lemma createObjects_ko_at:
   shows "\<lbrace>\<lambda>s. pspace_no_overlap' ptr sz s \<and> valid_pspace' s\<rbrace>
              createObjects ptr n ko gbits
          \<lbrace>\<lambda>r s. \<forall>x \<in> set r. \<forall>offs < 2 ^ gbits. ko_at' val (x + (offs << objBitsKO ko)) s\<rbrace>"
-  by (wp createObjects_ko_at_strg[OF cover not_0 pi],fastforce)
+  by (wp createObjects_ko_at_strg[OF cover not_0 pi], fastforce simp: valid_pspace'_def)
 
 lemma createObjects_obj_at:
   fixes ptr :: machine_word and val :: "'a :: pspace_storable"
@@ -2249,6 +2301,27 @@ lemma objBits_if_dev:
     "objBitsKO (if dev then KOUserDataDevice else KOUserData) = pageBits"
   by (simp add: objBitsKO_def)
 
+lemma createObjects_sc_at'_n:
+  fixes ptr :: machine_word and val :: sched_context
+  assumes  cover:"range_cover ptr sz ((objBitsKO ko) + gbits) n"
+  and      not_0:"n \<noteq> 0"
+  and       pi: "\<exists>(val::sched_context). projectKO_opt ko = Some val"
+  shows
+  "\<lbrace>\<lambda>s. pspace_no_overlap' ptr sz s \<and> valid_pspace' s\<rbrace>
+   createObjects ptr n ko gbits
+   \<lbrace>\<lambda>r s. \<forall>x \<in> set r. \<forall>offs < 2 ^ gbits.
+                         sc_at'_n (objBitsKO ko) (x + (offs << objBitsKO ko)) s\<rbrace>"
+  apply (rule exE[OF pi])
+  apply (prop_tac "objBitsKO ko = objBits x")
+   apply (clarsimp simp: objBits_def)
+  apply (erule_tac val1 = x in
+            hoare_post_imp [OF _ createObjects_ko_at [OF cover not_0 ],rotated])
+  apply (intro allI ballI impI)
+  apply (drule(1) bspec)
+  apply (drule spec, drule(1) mp)
+  apply (clarsimp simp: ko_wp_at'_def obj_at'_def objBits_def)
+  done
+
 lemma cwo_ret:
   assumes not_0: "n \<noteq> 0"
   assumes cover: "range_cover ptr sz (pageBits + bs) n"
@@ -2304,6 +2377,7 @@ lemma createNewCaps_valid_cap:
   assumes not_0: "n \<noteq> 0"
   assumes ct: "ty = APIObjectType ArchTypes_H.CapTableObject \<Longrightarrow> 0 < us"
               "ty = APIObjectType apiobject_type.Untyped \<Longrightarrow> minUntypedSizeBits \<le> us \<and> us \<le> maxUntypedSizeBits"
+              "ty = APIObjectType ArchTypes_H.SchedContextObject \<Longrightarrow> sc_size_bounds us"
   assumes ptr: "ptr \<noteq> 0"
 
   assumes ptr_cn: "canonical_address (ptr && ~~ mask sz)"
@@ -2413,15 +2487,16 @@ proof -
                              fromIntegral_def toInteger_nat fromInteger_nat APIType_capBits_def curDomain_def
                       split: RISCV64_H.object_type.splits)
         apply (wp mapM_x_wp' hoare_vcg_const_Ball_lift)+
-        apply (rule hoare_post_imp)
-         prefer 2
-         apply (rule createObjects_obj_at [where 'a = "tcb",OF _ not_0])
-          using cover
-          apply (clarsimp simp: RISCV64_H.toAPIType_def APIType_capBits_def objBits_simps
-                         split: RISCV64_H.object_type.splits)
-         apply simp
-        apply (clarsimp simp: valid_cap'_def objBits_simps)
-        apply (fastforce intro: capAligned_tcbI)
+         apply (rule hoare_post_imp)
+          prefer 2
+          apply (rule createObjects_obj_at [where 'a = "tcb",OF _ not_0])
+           using cover
+           apply (clarsimp simp: RISCV64_H.toAPIType_def APIType_capBits_def objBits_simps
+                          split: RISCV64_H.object_type.splits)
+           apply simp+
+         apply (clarsimp simp: valid_cap'_def objBits_simps)
+         apply (fastforce intro: capAligned_tcbI)
+        apply wp
         done
     next
       case EndpointObject with Some cover ct show ?thesis
@@ -2494,16 +2569,56 @@ proof -
          apply (clarsimp simp add: shiftl_t2n)
         apply simp
         done
+    next
+      case ReplyObject with Some cover ct show ?thesis
+        including no_pre
+        apply (clarsimp simp: Arch_createNewCaps_def createNewCaps_def)
+        apply (simp_all add: RISCV64_H.toAPIType_def
+                             fromIntegral_def toInteger_nat fromInteger_nat APIType_capBits_def
+                      split: RISCV64_H.object_type.splits)
+        apply wp
+        apply (rule hoare_post_imp)
+         prefer 2
+         apply (rule createObjects_obj_at [where 'a=reply, OF _ not_0])
+        using cover
+          apply (clarsimp simp: RISCV64_H.toAPIType_def objBits_simps
+                         split: RISCV64_H.object_type.splits)
+         apply simp
+        apply (simp add: valid_cap'_def)
+        apply (clarsimp simp: valid_cap'_def objBits_simps)
+        apply (fastforce intro: capAligned_replyI)
+        done
+    next
+      case SchedContextObject with Some cover ct show ?thesis
+        including no_pre
+        apply (clarsimp simp: Arch_createNewCaps_def createNewCaps_def)
+        apply (simp_all add: RISCV64_H.toAPIType_def
+                             fromIntegral_def toInteger_nat fromInteger_nat APIType_capBits_def
+                      split: RISCV64_H.object_type.splits)
+        apply wp
+        apply (rule hoare_post_imp)
+         prefer 2
+         apply (rule createObjects_sc_at'_n [OF _ not_0])
+        using cover ct(3)
+          apply (clarsimp simp: RISCV64_H.toAPIType_def objBits_simps APIType_capBits_def scBits_simps
+                         split: RISCV64_H.object_type.splits
+                         dest!: ct(3))
+         apply simp
+        apply (clarsimp, drule bspec, simp)
+        apply (prop_tac "sc_at'_n us cap s")
+         apply (clarsimp simp: objBitsKO_def scBits_simps)
+        apply (clarsimp simp: valid_cap'_def capAligned_sched_contextI sc_size_bounds_def)
+        done
     qed
   qed
 qed
 
 lemma other_objs_default_relation:
   "\<lbrakk> case ty of Structures_A.EndpointObject \<Rightarrow> ko = injectKO (makeObject :: endpoint)
-             | Structures_A.NotificationObject \<Rightarrow> ko = injectKO (makeObject :: Structures_H.notification)
-             | Structures_A.TCBObject \<Rightarrow> ko = injectKO (makeObject :: tcb)
-             | _ \<Rightarrow> False \<rbrakk> \<Longrightarrow>
-    obj_relation_retype (default_object ty dev n) ko"
+             | Structures_A.NotificationObject \<Rightarrow> ko = injectKO (makeObject :: notification)
+             | Structures_A.TCBObject \<Rightarrow> ko = injectKO (tcbDomain_update (\<lambda>_. d) makeObject)
+                          | _ \<Rightarrow> False \<rbrakk> \<Longrightarrow>
+    obj_relation_retype (default_object ty dev n d) ko"
   apply (rule obj_relation_retype_other_obj)
    apply (clarsimp simp: default_object_def
                          is_other_obj_relation_type_def
@@ -2515,7 +2630,7 @@ lemma other_objs_default_relation:
                         default_ep_def makeObject_endpoint default_notification_def
                         makeObject_notification default_ntfn_def
                         fault_rel_optionation_def
-                        initContext_def
+                        initContext_def default_priority_def
                         arch_tcb_context_get_def atcbContextGet_def
                         default_arch_tcb_def newArchTCB_def
                         arch_tcb_relation_def
@@ -2524,7 +2639,7 @@ lemma other_objs_default_relation:
 
 lemma captable_relation_retype:
   "n < word_bits \<Longrightarrow>
-   obj_relation_retype (default_object Structures_A.CapTableObject dev n) (KOCTE makeObject)"
+   obj_relation_retype (default_object Structures_A.CapTableObject dev n d) (KOCTE makeObject)"
   apply (clarsimp simp: obj_relation_retype_def default_object_def
                         wf_empty_bits objBits_simps'
                         dom_empty_cnode ex_with_length cte_level_bits_def)
@@ -2541,16 +2656,36 @@ lemma captable_relation_retype:
   apply (simp add: less_mask_eq)
   done
 
+lemma reply_relation_retype:
+  "obj_relation_retype (default_object Structures_A.ReplyObject dev n d)
+                                 (KOReply makeObject)"
+  by (simp add: default_object_def reply_relation_def default_reply_def
+                makeObject_reply obj_relation_retype_def
+                objBits_simps word_bits_def replySizeBits_def)
+
+lemma refillAbsoluteMax'_gt1:
+  "minSchedContextBits \<le> n \<Longrightarrow> min (Suc 0) (refillAbsoluteMax' n) = Suc 0"
+  by (drule refillAbsoluteMax'_lb) (simp add: minRefillLength_ARM)
+
+lemma sc_relation_retype:
+  "\<lbrakk>sc_size_bounds n\<rbrakk> \<Longrightarrow>
+   obj_relation_retype (default_object Structures_A.SchedContextObject dev n d)
+                         (KOSchedContext (scRefills_update
+                            (\<lambda>_. replicate (refillAbsoluteMax' n) emptyRefill) makeObject))"
+  by (clarsimp simp: default_object_def sc_relation_def default_sched_context_def
+                     makeObject_sc obj_relation_retype_def valid_sched_context_size_def
+                     objBits_simps word_bits_def scBits_simps refills_map_def refill_map_def
+                     emptyRefill_def refillAbsoluteMax'_gt1)
+
 lemma pagetable_relation_retype:
-  "obj_relation_retype (default_object (ArchObject PageTableObj) dev n)
+  "obj_relation_retype (default_object (ArchObject PageTableObj) dev n d)
                        (KOArch (KOPTE makeObject))"
-  apply (simp add: default_object_def default_arch_object_def
-                   makeObject_pte obj_relation_retype_def
+  apply (simp add: default_object_def default_arch_object_def makeObject_pte obj_relation_retype_def
                    objBits_simps pte_relation_def)
   apply (clarsimp simp: range_composition[symmetric]
                         shiftl_t2n field_simps)
   apply (subst image_comp [symmetric, where g=ucast, unfolded o_def])
-  apply (simp add: ucast_range_less)
+  apply (simp add: ucast_range_less pteBits_def)
   apply (fastforce simp: bit_simps)
   done
 
@@ -2558,30 +2693,31 @@ lemmas makeObjectKO_simps = makeObjectKO_def[split_simps RISCV64_H.object_type.s
  apiobject_type.split sum.split kernel_object.split ]
 
 lemma corres_retype:
-  assumes         not_zero: "n \<noteq> 0"
+  assumes    not_zero: "n \<noteq> 0"
   and         aligned: "is_aligned ptr (objBitsKO ko + gbits)"
   and    obj_bits_api: "obj_bits_api (APIType_map2 ty) us = objBitsKO ko + gbits"
   and              tp: "APIType_map2 ty \<in> no_gs_types"
-  and              ko: "makeObjectKO dev ty = Some ko"
+  and              ko: "makeObjectKO dev us d ty = Some ko"
+  and            tysc: "ty = Inr (APIObjectType SchedContextObject) \<longrightarrow> min_sched_context_bits \<le> us"
   and             orr: "obj_bits_api (APIType_map2 ty) us \<le> sz \<Longrightarrow>
-                        obj_relation_retype (default_object (APIType_map2 ty) dev us) ko"
+                        obj_relation_retype (default_object (APIType_map2 ty) dev us d) ko"
   and           cover: "range_cover ptr sz (obj_bits_api (APIType_map2 ty) us) n"
   shows "corres (=)
   (\<lambda>s. valid_pspace s \<and> pspace_no_overlap_range_cover ptr sz s
-     \<and> valid_mdb s \<and> valid_etcbs s \<and> valid_list s)
+     \<and> valid_mdb s \<and> valid_list s)
   (\<lambda>s. pspace_aligned' s \<and> pspace_distinct' s \<and> pspace_no_overlap' ptr sz s
-       \<and> (\<exists>val. ko = injectKO val))
-  (retype_region2 ptr n us (APIType_map2 ty) dev) (createObjects ptr n ko gbits)"
+       \<and> (\<exists>val. ko = injectKO val)
+       \<and> (ty = Inr (APIObjectType TCBObject) \<longrightarrow> d = ksCurDomain s))
+  (retype_region ptr n us (APIType_map2 ty) dev) (createObjects ptr n ko gbits)"
   apply (rule corres_guard_imp)
     apply (rule_tac F = "(\<exists>val. ko = injectKO val)" in corres_gen_asm2)
     apply (erule exE)
     apply (rule corres_rel_imp)
-    apply (rule corres_retype'[where g=id and ty=ty and sz = sz,OF not_zero aligned _ _ _ ko
+    apply (rule corres_retype'[where g=id and ty=ty and sz = sz,OF not_zero aligned _ _ ko
            ,simplified update_gs_id[OF tp] modify_id_return,simplified])
-        using assms
-        apply (simp_all add: objBits_def no_gs_types_def)
-  apply auto
-  done
+           using assms
+           apply (simp_all add: objBits_def no_gs_types_def)
+   by auto
 
 lemma init_arch_objects_APIType_map2:
   "init_arch_objects (APIType_map2 (Inr ty)) ptr bits sz refs =
@@ -2892,21 +3028,12 @@ lemma dist_z_n: "distinct_zombies n"
   apply (clarsimp simp: isCap_simps)
   done
 
-lemma reply_masters_rvk_fb_m: "reply_masters_rvk_fb m"
-  using valid by auto
-
-lemma reply_masters_rvk_fb_n: "reply_masters_rvk_fb n"
-  using reply_masters_rvk_fb_m
-  by (simp add: n_def reply_masters_rvk_fb_def
-                ball_ran_eq makeObject_cte isCap_simps)
-
 lemma valid_n:
   "valid_mdb_ctes n"
   by (simp add: valid_mdb_ctes_def dlist_n no_0_n mdb_chain_0_n
                 valid_badges_n caps_contained_n untyped_mdb_n
                 untyped_inc_n mdb_chunked_n valid_nullcaps_n ut_rev_n
-                class_links_n irq_control_n dist_z_n
-                reply_masters_rvk_fb_n)
+                class_links_n irq_control_n dist_z_n)
 
 end
 
@@ -2942,6 +3069,8 @@ proof -
       using not_0 n_less
       apply simp
       done
+    have bd[simp]: "objBitsKO val < word_bits"
+      using assms by (clarsimp simp: range_cover_def word_bits_def)
     have "ptr' + 2 ^ objBitsKO val - 1 \<le> ptr + of_nat n * 2 ^ objBitsKO val - 1"
       using cover including no_take_bit
       apply (subst decomp)
@@ -3007,55 +3136,59 @@ lemma valid_untyped'_helper:
   and  cover  : "range_cover ptr sz (objBitsKO val) n"
   and  range  : "caps_no_overlap'' ptr sz s"
   and  pres   : "isUntypedCap c \<longrightarrow> usableUntypedRange c \<inter>  {ptr..ptr + of_nat n * 2 ^ objBitsKO val - 1} = {}"
-  shows "\<lbrakk>pspace_aligned' s; pspace_distinct' s; pspace_no_overlap' ptr sz s\<rbrakk>
- \<Longrightarrow> valid_cap' c (s\<lparr>ksPSpace := foldr (\<lambda>addr. data_map_insert addr val) (new_cap_addrs n ptr val) (ksPSpace s)\<rparr>)"
-  proof -
-  note blah[simp del] = atLeastAtMost_iff atLeastatMost_subset_iff atLeastLessThan_iff
-        Int_atLeastAtMost atLeastatMost_empty_iff
-  assume pn : "pspace_aligned' s" "pspace_distinct' s"
-  and   no_overlap: "pspace_no_overlap' ptr sz s"
+  shows "\<lbrakk>pspace_aligned' s; pspace_distinct' s;  pspace_bounded' s; pspace_no_overlap' ptr sz s\<rbrakk>
+          \<Longrightarrow> valid_cap' c (s\<lparr>ksPSpace := foldr (\<lambda>addr. data_map_insert addr val)
+                                                      (new_cap_addrs n ptr val) (ksPSpace s)\<rparr>)"
+proof -
+  note blah[simp del] = atLeastAtMost_simps
+  note cover' = range_cover_rel[where sbit' = "objBitsKO val",OF cover _ refl,simplified]
+  assume pn : "pspace_aligned' s" "pspace_distinct' s" "pspace_bounded' s"
+  and no_overlap: "pspace_no_overlap' ptr sz s"
   show ?thesis
-  using pn pres no_overlap valid cover cte_wp_at_ctes_of[THEN iffD1,OF cte_at]
-        caps_no_overlapD''[OF cte_at range]
-  apply (clarsimp simp:valid_cap'_def retype_ko_wp_at')
-  apply (case_tac "cteCap cte";
-         simp add: valid_cap'_def cte_wp_at_obj_cases' valid_pspace'_def retype_obj_at_disj'
-            split: zombie_type.split_asm)
-   apply (clarsimp simp: valid_arch_cap'_def valid_arch_cap_ref'_def retype_obj_at_disj'
-                         typ_at_to_obj_at_arches frame_at'_def page_table_at'_def
-                   split: if_split_asm arch_capability.splits)
-  unfolding valid_untyped'_def
-  apply (intro allI)
-  apply (rule ccontr)
-  apply clarify
-  using cover[unfolded range_cover_def]
-  apply (clarsimp simp:isCap_simps retype_ko_wp_at' split:if_split_asm)
-   apply (thin_tac "\<forall>x. Q x" for Q)
-   apply (frule aligned_untypedRange_non_empty)
-    apply (simp add:isCap_simps)
-   apply (elim disjE)
-    apply (frule(1) obj_range'_subset)
-    apply (erule impE)
-     apply (drule(1) psubset_subset_trans)
-     apply (drule Int_absorb1[OF psubset_imp_subset])
-     apply (drule aligned_untypedRange_non_empty)
+    using pn pres no_overlap valid cover cte_wp_at_ctes_of[THEN iffD1,OF cte_at]
+      caps_no_overlapD''[OF cte_at range]
+    apply (clarsimp simp:valid_cap'_def retype_ko_wp_at')
+    apply (case_tac "cteCap cte"; simp add: valid_cap'_def cte_wp_at_obj_cases'
+                                  valid_pspace'_def retype_obj_at_disj' retype_ko_wp_at'
+                           split: zombie_type.split_asm)
+      apply (clarsimp simp: valid_arch_cap'_def valid_arch_cap_ref'_def retype_obj_at_disj'
+                            typ_at_to_obj_at_arches frame_at'_def page_table_at'_def
+                     split: if_split_asm arch_capability.splits)
+     unfolding valid_untyped'_def
+     apply (intro allI)
+     apply (rule ccontr)
+     apply clarify
+     using cover[unfolded range_cover_def]
+     apply (clarsimp simp:isCap_simps retype_ko_wp_at' split:if_split_asm)
+      apply (thin_tac "\<forall>x. Q x" for Q)
+      apply (frule aligned_untypedRange_non_empty)
       apply (simp add:isCap_simps)
-     apply (simp add:Int_ac add_mask_fold)
+     apply (elim disjE)
+      apply (frule(1) obj_range'_subset)
+      apply (erule impE)
+       apply (drule(1) psubset_subset_trans)
+       apply (drule Int_absorb1[OF psubset_imp_subset])
+       apply (drule aligned_untypedRange_non_empty)
+        apply (simp add:isCap_simps)
+       apply (simp add:Int_ac add_mask_fold)
+      apply (drule(1) subset_trans)
+      apply (simp only: add_mask_fold)
+     apply (frule(1) obj_range'_subset_strong)
+     apply (drule(1) non_disjoing_subset)
+     apply blast
+    apply (thin_tac "\<forall>x. Q x" for Q)
+    apply (frule aligned_untypedRange_non_empty)
+     apply (simp add:isCap_simps)
+    apply (frule(1) obj_range'_subset)
     apply (drule(1) subset_trans)
+    apply (erule impE)
+     apply (clarsimp simp: add_mask_fold)
+     apply blast
     apply (simp only: add_mask_fold)
-   apply (frule(1) obj_range'_subset_strong)
-   apply (drule(1) non_disjoing_subset)
-   apply blast
-  apply (thin_tac "\<forall>x. Q x" for Q)
-  apply (frule aligned_untypedRange_non_empty)
-   apply (simp add:isCap_simps)
-  apply (frule(1) obj_range'_subset)
-  apply (drule(1) subset_trans)
-  apply (erule impE)
-   apply (clarsimp simp: add_mask_fold)
-   apply blast
-  apply (simp only: add_mask_fold)
-  apply blast
+    apply blast
+   apply clarsimp
+   apply (drule (3) retype_ko_wp_at'_not[where gbits=0, simplified, OF _ _ _ cover])
+   apply (erule notE, simp)
   done
 qed
 
@@ -3101,8 +3234,10 @@ proof -
 qed
 
 lemma createObjects_valid_pspace':
-  assumes  mko: "makeObjectKO dev ty = Some val"
+  assumes  mko: "makeObjectKO dev us d ty = Some val"
+  and    max_d: "ty = Inr (APIObjectType TCBObject) \<longrightarrow> d \<le> maxDomain"
   and    not_0: "n \<noteq> 0"
+  and     tysc: "ty = Inr (APIObjectType SchedContextObject) \<longrightarrow> sc_size_bounds us"
   and    cover: "range_cover ptr sz (objBitsKO val + gbits) n"
   and    sz_limit: "sz \<le> maxUntypedSizeBits"
   and    ptr_cn: "canonical_address (ptr && ~~ mask sz)"
@@ -3110,7 +3245,8 @@ lemma createObjects_valid_pspace':
   shows "\<lbrace>\<lambda>s. pspace_no_overlap' ptr sz s \<and> valid_pspace' s \<and> caps_no_overlap'' ptr sz s
             \<and> caps_overlap_reserved' {ptr .. ptr + of_nat (n * 2^gbits * 2 ^ objBitsKO val ) - 1} s
             \<and> ptr \<noteq> 0\<rbrace>
-  createObjects' ptr n val gbits \<lbrace>\<lambda>r. valid_pspace'\<rbrace>"
+         createObjects' ptr n val gbits
+         \<lbrace>\<lambda>_. valid_pspace'\<rbrace>"
   apply (cut_tac not_0)
   apply (simp add: split_def createObjects'_def
                    lookupAround2_pspace_no
@@ -3139,7 +3275,9 @@ proof (intro conjI impI)
 
   assume pn: "pspace_no_overlap' ptr sz s"
      and vo: "valid_objs' s"
+     and vr: "valid_replies' s"
      and ad: "pspace_aligned' s" "pspace_distinct' s"
+     and bd: "pspace_bounded' s"
      and cn: "pspace_canonical' s"
      and km: "pspace_in_kernel_mappings' s"
      and pc: "caps_no_overlap'' ptr sz s"
@@ -3155,7 +3293,7 @@ proof (intro conjI impI)
 
   note cover' = range_cover_rel[where sbit' = "objBitsKO val",OF cover _ refl,simplified]
 
-  note ad' = retype_aligned_distinct'[OF ad pn cover']
+  note ad' = retype_aligned_distinct'[OF ad bd pn cover']
 
   note shift = range_cover.unat_of_nat_n_shift[OF cover,where gbits=gbits,simplified]
 
@@ -3179,7 +3317,7 @@ proof (intro conjI impI)
   using ad' shift
     by (simp add:field_simps)
 
-  note obj_at_disj = retype_obj_at_disj' [OF ad pn cover']
+  note obj_at_disj = retype_obj_at_disj' [OF ad bd pn cover']
 
   note obj_at_disj' = obj_at_disj [unfolded foldr_upd_app_if[folded data_map_insert_def]]
 
@@ -3194,7 +3332,7 @@ proof (intro conjI impI)
 
   have valid_cap: "\<And>cap q. \<lbrakk> s \<turnstile>' cap; cte_wp_at' (\<lambda>cte. cteCap cte = cap) q s \<rbrakk>
                       \<Longrightarrow> ?s' \<turnstile>' cap"
-     apply (rule valid_untyped'_helper[OF _ _ _ pc _ ad pn ])
+     apply (rule valid_untyped'_helper[OF _ _ _ pc _ ad bd pn ])
           apply simp+
         apply (subst mult.commute)
         apply (rule cover')
@@ -3205,13 +3343,13 @@ proof (intro conjI impI)
      apply simp
    done
 
-  show valid_objs: "valid_objs' ?s'" using vo
+  show valid_objs: "valid_objs' ?s'" using vo tysc
     apply (clarsimp simp: valid_objs'_def
                           foldr_upd_app_if[folded data_map_insert_def]
                    elim!: ranE
                    split: if_split_asm)
      apply (insert sym[OF mko])[1]
-     apply (clarsimp simp: makeObjectKO_def
+     apply (clarsimp simp: makeObjectKO_def max_d
                     split: bool.split_asm sum.split_asm
                            RISCV64_H.object_type.split_asm
                            apiobject_type.split_asm
@@ -3220,50 +3358,76 @@ proof (intro conjI impI)
     apply (drule bspec, erule ranI)
     apply (subst mult.commute)
     apply (case_tac obj; simp add: valid_obj'_def)
-       apply (rename_tac endpoint)
-       apply (case_tac endpoint; simp add: valid_ep'_def obj_at_disj')
-      apply (rename_tac notification)
-      apply (case_tac notification; simp add: valid_ntfn'_def valid_bound_tcb'_def obj_at_disj')
-      apply (rename_tac ntfn xa)
-      apply (case_tac ntfn, simp_all, (clarsimp simp: obj_at_disj' split:option.splits)+)
-     apply (rename_tac tcb)
-     apply (case_tac tcb, clarsimp simp add: valid_tcb'_def)
-     apply (frule pspace_alignedD' [OF _ ad(1)])
-     apply (frule pspace_distinctD' [OF _ ad(2)])
-     apply (simp add: objBits_simps)
-     apply (subst mult.commute)
-     apply (intro conjI ballI)
-       apply (clarsimp elim!: ranE)
-       apply (rule valid_cap[unfolded foldr_upd_app_if[folded data_map_insert_def]])
-        apply (fastforce)
-       apply (rule_tac ptr="x + xa" in cte_wp_at_tcbI', assumption+)
-        apply fastforce
-       apply simp
-      apply (rename_tac thread_state mcp priority bool option nat cptr vptr bound user_context)
-      apply (case_tac thread_state, simp_all add: valid_tcb_state'_def
-                                                  valid_bound_ntfn'_def obj_at_disj'
-                                           split: option.splits)[2]
-    apply (simp add: valid_cte'_def)
-    apply (frule pspace_alignedD' [OF _ ad(1)])
-    apply (frule pspace_distinctD' [OF _ ad(2)])
-    apply (simp add: objBits_simps')
-    apply (subst mult.commute)
-    apply (erule valid_cap[unfolded foldr_upd_app_if[folded data_map_insert_def]])
-    apply (erule(2) cte_wp_at_cteI'[unfolded cte_level_bits_def])
-    apply simp
+         apply (rename_tac endpoint)
+         apply (case_tac endpoint; simp add: valid_ep'_def obj_at_disj')
+        apply (rename_tac notification)
+        apply (case_tac notification; simp add: valid_ntfn'_def valid_bound_tcb'_def obj_at_disj')
+        apply (rename_tac ntfn xa xb)
+        apply (case_tac ntfn, simp_all, (clarsimp simp: obj_at_disj' split:option.splits)+)
+       apply (rename_tac tcb)
+       apply (case_tac tcb, clarsimp simp add: valid_tcb'_def)
+       apply (frule pspace_alignedD' [OF _ ad(1)])
+       apply (frule pspace_distinctD' [OF _ ad(2)])
+       apply (simp add: objBits_simps)
+       apply (subst mult.commute)
+       apply (intro conjI ballI)
+           apply (clarsimp elim!: ranE)
+           apply (rule valid_cap[unfolded foldr_upd_app_if[folded data_map_insert_def]])
+            apply fastforce
+           apply (rule_tac ptr="x + xa" in cte_wp_at_tcbI', assumption+)
+           apply fastforce
+          apply simp
+          apply (rename_tac thread_state mcp priority inQ inRQ option vptr bound tcbsc tcbyt user_context)
+          apply (case_tac thread_state, simp_all add: valid_tcb_state'_def
+                                                      valid_bound_ntfn'_def obj_at_disj'
+                                               split: option.splits)[4]
+      apply (simp add: valid_cte'_def)
+      apply (frule pspace_alignedD' [OF _ ad(1)])
+      apply (frule pspace_distinctD' [OF _ ad(2)])
+      apply (simp add: objBits_simps')
+      apply (subst mult.commute)
+      apply (erule valid_cap[unfolded foldr_upd_app_if[folded data_map_insert_def]])
+      apply (erule(2) cte_wp_at_cteI'[unfolded cte_level_bits_def])
+      apply simp
+     apply (rename_tac sc)
+     apply (case_tac sc; simp add: valid_sched_context'_def valid_bound_tcb'_def obj_at_disj'
+                            split: option.splits)
+    apply (rename_tac reply)
+    apply (case_tac reply; fastforce simp: valid_reply'_def valid_bound_tcb'_def obj_at_disj'
+                    split: option.splits)
     done
+
+  show valid_replies': "valid_replies' ?s'" using vr
+    apply (subst mult.commute)
+    apply (clarsimp simp: valid_replies'_def pred_tcb_at'_def obj_at_disj'
+                          foldr_upd_app_if[folded data_map_insert_def]
+                   elim!: ranE
+                   split: if_split_asm)
+    apply (insert sym[OF mko])[1]
+    apply (clarsimp simp: makeObjectKO_def projectKOs opt_map_def makeObject_reply
+                   split: bool.split_asm sum.split_asm
+                          RISCV64_H.object_type.split_asm
+                          apiobject_type.split_asm
+                          kernel_object.split_asm
+                          arch_kernel_object.split_asm
+                          if_splits option.splits)
+    apply fastforce
+    done
+
   have not_0: "0 \<notin> set (new_cap_addrs (2 ^ gbits * n) ptr val)"
     using p_0
     apply clarsimp
     apply (drule subsetD [OF new_cap_addrs_subset [OF cover'],rotated])
     apply (clarsimp simp:ptr_add_def)
     done
+
   show "valid_mdb' ?s'"
     apply (simp add: valid_mdb'_def foldr_upd_app_if[folded data_map_insert_def])
     apply (subst mult.commute)
     apply (subst ctes_of_retype [OF mko ad])
         apply (rule ad'[unfolded foldr_upd_app_if[folded data_map_insert_def]])+
       apply (simp add: objBits_def[symmetric] new_cap_addrs_aligned [OF al])
+      using cover apply (clarsimp simp: range_cover_def word_bits_def)
      apply (rule ballI, drule subsetD [OF new_cap_addrs_subset [OF cover']])
      apply (insert pspace_no_overlap_disjoint' [OF ad(1) pn])
      apply (drule_tac x = x in orthD1)
@@ -3312,14 +3476,20 @@ proof (intro conjI impI)
     using not_0 no_0_obj'
     by (simp add: no_0_obj'_def data_map_ext field_simps foldr_upd_app_other)
 
+  show bounded': "pspace_bounded' ?s'"
+  using ad' shift range_cover.unat_of_nat_n_shift[OF cover,where gbits=gbits,simplified]
+    by (simp add: field_simps)
+
 qed
 
 abbreviation
  "injectKOS \<equiv> (injectKO :: ('a :: pspace_storable) \<Rightarrow> kernel_object)"
 
 lemma createObjects_valid_pspace_untyped':
-  assumes  mko: "makeObjectKO dev ty = Some val"
+  assumes  mko: "makeObjectKO dev us d ty = Some val"
+  and    max_d: "ty = Inr (APIObjectType TCBObject) \<longrightarrow> d \<le> maxDomain"
   and    not_0: "n \<noteq> 0"
+  and     tysc: "ty = Inr (APIObjectType SchedContextObject) \<longrightarrow> sc_size_bounds us"
   and    cover: "range_cover ptr sz (objBitsKO val + gbits) n"
   and    sz_limit: "sz \<le> maxUntypedSizeBits"
   and    ptr_cn: "canonical_address (ptr && ~~ mask sz)"
@@ -3327,34 +3497,33 @@ lemma createObjects_valid_pspace_untyped':
   shows "\<lbrace>\<lambda>s. pspace_no_overlap' ptr sz s \<and> valid_pspace' s \<and> caps_no_overlap'' ptr sz s \<and> ptr \<noteq> 0
             \<and> caps_overlap_reserved' {ptr .. ptr + of_nat (n * 2^gbits * 2 ^ objBitsKO val ) - 1} s \<rbrace>
   createObjects' ptr n val gbits \<lbrace>\<lambda>r. valid_pspace'\<rbrace>"
-  apply (wp createObjects_valid_pspace' [OF mko not_0 cover sz_limit ptr_cn ptr_km])
-  apply simp
-  done
+  using assms
+  by (wpsimp wp: createObjects_valid_pspace' [OF mko max_d not_0 tysc cover])
 
-lemma copyGlobalMappings_valid_objs'[wp]:
-  "copyGlobalMappings pt \<lbrace>valid_objs'\<rbrace>"
-  unfolding copyGlobalMappings_def by (wpsimp wp: mapM_x_wp')
-
-crunch pspace_aligned'[wp]: copyGlobalMappings "pspace_aligned'"
-  (wp: crunch_wps)
-crunch pspace_canonical'[wp]: copyGlobalMappings "pspace_canonical'"
-  (wp: crunch_wps)
-crunch pspace_in_kernel_mappings'[wp]: copyGlobalMappings "pspace_in_kernel_mappings'"
-  (wp: crunch_wps)
-crunch pspace_distinct'[wp]: copyGlobalMappings "pspace_distinct'"
+crunches copyGlobalMappings
+  for valid_objs'[wp]: valid_objs'
+  and pspace_aligned'[wp]: pspace_aligned'
+  and pspace_distinct'[wp]: pspace_distinct'
+  and pspace_canonical'[wp]: pspace_canonical'
+  and pspace_bounded'[wp]: pspace_bounded'
+  and pspace_in_kernel_mappings'[wp]: pspace_in_kernel_mappings'
+  and valid_mdb[wp]: valid_mdb'
+  and no_0_obj' [wp]: no_0_obj'
   (wp: crunch_wps)
 
 lemmas storePTE_valid_mdb[wp]
-    = storePTE_ctes[where P=valid_mdb_ctes, folded valid_mdb'_def]
-crunch valid_mdb[wp]: copyGlobalMappings "valid_mdb'"
-  (wp: crunch_wps)
+    = storePTE.ctes_of[where P=valid_mdb_ctes, folded valid_mdb'_def]
 
-crunch no_0_obj' [wp]: copyGlobalMappings no_0_obj'
-  (wp: crunch_wps)
+lemma copyGlobalMappings_valid_replies'[wp]:
+  "\<lbrace>valid_replies' and pspace_aligned' and pspace_distinct'\<rbrace>
+   copyGlobalMappings pd
+   \<lbrace>\<lambda>_. valid_replies'\<rbrace>" (is "\<lbrace>?Pre\<rbrace> _ \<lbrace>_\<rbrace>")
+  unfolding copyGlobalMappings_def
+  by (wpsimp wp: mapM_x_inv_wp[where I="?Pre"])
 
-lemma copyGlobalMappings_valid_pspace[wp]:
-  "\<lbrace>valid_pspace'\<rbrace> copyGlobalMappings pt \<lbrace>\<lambda>rv. valid_pspace'\<rbrace>"
-  by (wpsimp simp: valid_pspace'_def)
+lemma copyGlobalMappings_valid_pspace'[wp]:
+  "\<lbrace>valid_pspace'\<rbrace> copyGlobalMappings pd \<lbrace>\<lambda>rv. valid_pspace'\<rbrace>"
+  by (simp add: valid_pspace'_def | wp)+
 
 declare bleeding_obvious [simp]
 
@@ -3367,8 +3536,11 @@ proof -
   note unat_of_nat_shift = range_cover.unat_of_nat_n_shift[OF cover,where gbits=gbits,simplified]
   have cover' :"range_cover ptr sz (objBitsKO val) (n*2^gbits)"
     by (rule range_cover_rel[OF cover],simp+)
+  have bd: "objBitsKO val < word_bits"
+    using cover
+    by (simp add: range_cover_def word_bits_def)
   have upbound:" unat ((((of_nat n)::machine_word) * 2 ^ gbits)) * unat ((2::machine_word) ^ objBitsKO val) < 2 ^ word_bits"
-    using range_cover.range_cover_le_n_less[OF cover' le_refl] cover'
+    using range_cover.range_cover_le_n_less[OF cover' le_refl] cover' bd
     apply -
       apply (drule nat_less_power_trans)
        apply (simp add:range_cover_def)
@@ -3387,7 +3559,7 @@ proof -
   thus ?thesis
   including no_take_bit
   apply -
-  apply (insert not_0 cover ptr_in)
+  apply (insert not_0 cover ptr_in bd)
   apply (frule range_cover.range_cover_le_n_less[OF _ le_refl])
   apply (fold word_bits_def)
   apply (simp add:shiftL_nat )
@@ -3427,7 +3599,7 @@ proof -
       apply (rule word_of_nat_less)
       using unat_of_nat_shift
       apply (simp add:shiftl_t2n field_simps)
-     apply (meson less_exp objBitsKO_bounded2 of_nat_less_pow_64 word_gt_a_gt_0)
+     apply (meson less_exp of_nat_less_pow_64 word_gt_a_gt_0)
    using upbound
    apply (simp add:word_bits_def)
    apply (rule machine_word_plus_mono_right_split[where sz = sz])
@@ -3442,7 +3614,7 @@ qed
 
 lemma createObjects_orig_ko_wp_at2':
   "\<lbrace>\<lambda>s. range_cover ptr sz (objBitsKO val + gbits) n \<and> n \<noteq> 0
-      \<and> pspace_aligned' s \<and> pspace_distinct' s
+      \<and> pspace_aligned' s \<and> pspace_distinct' s \<and> pspace_bounded' s
       \<and> P (ko_wp_at' P' p s)
       \<and> (P' val \<longrightarrow> P True)
       \<and> pspace_no_overlap' ptr sz s\<rbrace>
@@ -3489,7 +3661,7 @@ lemma createObjects_orig_ko_wp_at2':
 lemma createObjects_orig_obj_at2':
   "\<lbrace>\<lambda>s. n \<noteq> 0
       \<and> range_cover ptr sz (objBitsKO val + gbits) n
-      \<and> pspace_aligned' s \<and> pspace_distinct' s
+      \<and> pspace_aligned' s \<and> pspace_distinct' s \<and> pspace_bounded' s
       \<and> P (obj_at' P' p s)
       \<and> \<not> (case_option False P' (projectKO_opt val))
       \<and> pspace_no_overlap' ptr sz s\<rbrace>
@@ -3501,7 +3673,7 @@ lemma createObjects_orig_cte_wp_at2':
   "\<lbrace>\<lambda>s. P (cte_wp_at' P' p s)
       \<and> n \<noteq> 0
       \<and> range_cover ptr sz (objBitsKO val + gbits) n
-      \<and> pspace_aligned' s \<and> pspace_distinct' s
+      \<and> pspace_aligned' s \<and> pspace_distinct' s \<and> pspace_bounded' s
       \<and> \<not> (case_option False P' (projectKO_opt val))
       \<and> (\<forall>(getF, setF) \<in> ran tcb_cte_cases.
               \<not> (case_option False (P' \<circ> getF) (projectKO_opt val)))
@@ -3527,8 +3699,10 @@ lemmas threadSet_cte_wp_at2' =
 lemma createNewCaps_cte_wp_at2:
   "\<lbrace>\<lambda>s. P (cte_wp_at' P' p s) \<and> \<not> P' makeObject
       \<and> n \<noteq> 0
+      \<and> (ty = APIObjectType ArchTypes_H.apiobject_type.SchedContextObject
+               \<longrightarrow> minSchedContextBits \<le> objsz)
       \<and> range_cover ptr sz (APIType_capBits ty objsz) n
-      \<and> pspace_aligned' s \<and> pspace_distinct' s
+      \<and> pspace_aligned' s \<and> pspace_distinct' s \<and> pspace_bounded' s
       \<and> pspace_no_overlap' ptr sz s\<rbrace>
      createNewCaps ty ptr n objsz dev
    \<lbrace>\<lambda>rv s. P (cte_wp_at' P' p s)\<rbrace>"
@@ -3539,23 +3713,21 @@ lemma createNewCaps_cte_wp_at2:
                            split del: if_split cong: if_cong)
         apply (rename_tac apiobject_type)
         apply (case_tac apiobject_type; simp split del: if_split)
-            apply (rule hoare_pre, wp, simp add:createObjects_def)
-           apply ((wp createObjects_orig_cte_wp_at2'[where sz = sz]
-                     mapM_x_wp' threadSet_cte_wp_at2')+
-                   | assumption
-                   | clarsimp simp: APIType_capBits_def projectKO_opts_defs
-                                    makeObject_tcb tcb_cte_cases_def cteSizeBits_def
-                                    archObjSize_def bit_simps
-                                    createObjects_def curDomain_def
-                                    objBits_if_dev
-                         split del: if_split
-                   | simp add: objBits_simps)+
-  done
+              apply (rule hoare_pre, wp, simp add:createObjects_def)
+  by (wpsimp wp: createObjects_orig_cte_wp_at2'[where sz = sz] mapM_x_wp' split_del: if_split
+           simp: createObjects_def curDomain_def objBits_simps APIType_capBits_def
+      | simp add: projectKO_opts_defs makeObject_tcb tcb_cte_cases_def Let_def
+                  scBits_simps objBits_if_dev objBits_simps
+                  archObjSize_def   ptBits_def pteBits_def pageBits_def objBits_simps'
+                  pt_bits_def pte_bits_def word_size_bits_def table_size_def
+                  ptTranslationBits_def
+       split del: if_split
+      | simp)+
 
 lemma createObjects_orig_obj_at':
   "\<lbrace>\<lambda>s. n \<noteq> 0
       \<and> range_cover ptr sz (objBitsKO val + gbits) n
-      \<and> pspace_aligned' s \<and> pspace_distinct' s
+      \<and> pspace_aligned' s \<and> pspace_distinct' s \<and> pspace_bounded' s
       \<and> obj_at' P p s
       \<and> pspace_no_overlap' ptr sz s\<rbrace>
    createObjects' ptr n val gbits \<lbrace>\<lambda>r. obj_at' P p\<rbrace>"
@@ -3600,7 +3772,7 @@ crunch ko_wp_at'[wp]: doMachineOp "\<lambda>s. P (ko_wp_at' P' p s)"
 
 lemma createObjects_orig_cte_wp_at':
   "\<lbrace>\<lambda>s. range_cover ptr sz (objBitsKO val + gbits) n \<and> n \<noteq> 0
-      \<and> pspace_aligned' s \<and> pspace_distinct' s
+      \<and> pspace_aligned' s \<and> pspace_distinct' s \<and> pspace_bounded' s
       \<and> cte_wp_at' P p s
       \<and> pspace_no_overlap' ptr sz s\<rbrace>
   createObjects' ptr n val gbits \<lbrace>\<lambda>r s. cte_wp_at' P p s\<rbrace>"
@@ -3612,7 +3784,9 @@ lemma createObjects_orig_cte_wp_at':
 lemma createNewCaps_cte_wp_at':
   "\<lbrace>\<lambda>s. cte_wp_at' P p s
       \<and> range_cover ptr sz (APIType_capBits ty us) n \<and> n \<noteq> 0
-      \<and> pspace_aligned' s \<and> pspace_distinct' s
+      \<and> (ty = APIObjectType ArchTypes_H.apiobject_type.SchedContextObject
+               \<longrightarrow> sc_size_bounds us)
+      \<and> pspace_aligned' s \<and> pspace_distinct' s \<and> pspace_bounded' s
       \<and> pspace_no_overlap' ptr sz s\<rbrace>
      createNewCaps ty ptr n us dev
    \<lbrace>\<lambda>rv. cte_wp_at' P p\<rbrace>"
@@ -3626,7 +3800,7 @@ lemma createNewCaps_cte_wp_at':
            apply (wp createObjects_orig_cte_wp_at'[where sz = sz] mapM_x_wp'
                      threadSet_cte_wp_at'T
                   | clarsimp simp: objBits_simps APIType_capBits_def createObjects_def curDomain_def
-                                   bit_simps
+                                   bit_simps scBits_simps
                   | intro conjI impI
                   | force simp: tcb_cte_cases_def cteSizeBits_def)+
   done
@@ -3653,44 +3827,42 @@ lemma valid_cap'_range_no_overlap:
                             typ_at_to_obj_at_arches frame_at'_def page_table_at'_def
                        split: zombie_type.split_asm arch_capability.splits if_splits
                        del: Int_atLeastAtMost)[1]
-  apply (rename_tac word nat1 nat2)
-  apply (clarsimp simp:valid_untyped'_def retype_ko_wp_at'
-        simp del: atLeastAtMost_iff atLeastatMost_subset_iff atLeastLessThan_iff
-        Int_atLeastAtMost atLeastatMost_empty_iff)
-  apply (frule aligned_untypedRange_non_empty)
-   apply (simp add:isCap_simps)
-  apply (intro conjI impI)
+   apply (rename_tac word nat1 nat2)
+   apply (clarsimp simp: valid_untyped'_def retype_ko_wp_at'
+               simp del: atLeastAtMost_simps)
+   apply (frule aligned_untypedRange_non_empty)
+    apply (simp add:isCap_simps)
+   apply (intro conjI impI)
+    apply (intro allI)
+    apply (drule_tac x = ptr' in spec)
+    apply (rule ccontr)
+    apply (clarsimp simp del: atLeastAtMost_simps)
+    apply (erule disjE)
+     apply (drule(2) disjoint_subset2 [OF obj_range'_subset])
+     apply (drule(1) disjoint_subset2[OF psubset_imp_subset])
+     apply (simp add: Int_absorb ptr_add_def p_assoc_help mask_def
+                 del: atLeastAtMost_simps)
+    apply (drule(1) obj_range'_subset)
+    apply (drule_tac A'=" {word + of_nat nat2..word + 2 ^ nat1 - 1}" in disjoint_subset[rotated])
+     apply clarsimp
+     apply (rule is_aligned_no_wrap')
+      apply (fastforce simp:capAligned_def)
+     apply (erule of_nat_less_pow_64)
+     apply (simp add:capAligned_def)
+    apply (drule(1) disjoint_subset2)
+    apply (simp add: add_mask_fold)
+    apply blast
    apply (intro allI)
    apply (drule_tac x = ptr' in spec)
    apply (rule ccontr)
-   apply (clarsimp simp del: atLeastAtMost_iff atLeastatMost_subset_iff atLeastLessThan_iff
-                             Int_atLeastAtMost atLeastatMost_empty_iff)
-   apply (erule disjE)
-    apply (drule(2) disjoint_subset2 [OF obj_range'_subset])
-    apply (drule(1) disjoint_subset2[OF psubset_imp_subset])
-    apply (simp add: Int_absorb ptr_add_def p_assoc_help mask_def
-                del: atLeastAtMost_iff atLeastatMost_subset_iff atLeastLessThan_iff
-                     Int_atLeastAtMost atLeastatMost_empty_iff)
-   apply (drule(1) obj_range'_subset)
-   apply (drule_tac A'=" {word + of_nat nat2..word + 2 ^ nat1 - 1}" in disjoint_subset[rotated])
-    apply clarsimp
-    apply (rule is_aligned_no_wrap')
-     apply (fastforce simp:capAligned_def)
-    apply (erule of_nat_less_pow_64)
-    apply (simp add:capAligned_def)
+   apply (clarsimp simp del: atLeastAtMost_simps)
+   apply (drule(2) disjoint_subset2 [OF obj_range'_subset])
    apply (drule(1) disjoint_subset2)
-   apply (simp add: add_mask_fold)
-   apply blast
-  apply (intro allI)
-  apply (drule_tac x = ptr' in spec)
-  apply (rule ccontr)
-  apply (clarsimp simp del: atLeastAtMost_iff atLeastatMost_subset_iff atLeastLessThan_iff
-                            Int_atLeastAtMost atLeastatMost_empty_iff)
-  apply (drule(2) disjoint_subset2 [OF obj_range'_subset])
-  apply (drule(1) disjoint_subset2)
-  apply (simp add: Int_absorb ptr_add_def p_assoc_help mask_def
-              del: atLeastAtMost_iff atLeastatMost_subset_iff atLeastLessThan_iff
-                   Int_atLeastAtMost atLeastatMost_empty_iff)
+   apply (simp add: Int_absorb ptr_add_def p_assoc_help mask_def
+               del: atLeastAtMost_simps)
+  apply (clarsimp simp: retype_ko_wp_at')
+  apply (drule (4) retype_ko_wp_at'_not[where gbits=0, simplified])
+  apply (erule notE, simp)
   done
 
 lemma createObjects_valid_cap':
@@ -3733,24 +3905,26 @@ lemma createObjects_cte_wp_at':
   apply (erule disjE)
    apply (erule use_valid[OF _ ])
     apply (rule createObjects_orig_obj_at')
-   apply fastforce
+   apply (fastforce simp: valid_pspace'_def)
   apply clarsimp
   apply (drule_tac x = na in bspec)
    apply clarsimp
   apply clarsimp
   apply (drule use_valid[OF _ createObjects_orig_obj_at'])
-   apply fastforce
+   apply (fastforce simp: valid_pspace'_def)
   apply simp
   done
 
 lemma createNewCaps_cte_wp_at:
   assumes cover: "range_cover ptr sz (APIType_capBits ty us) n"
   and not_0 : "n \<noteq> 0"
+  and  tysc : "ty = APIObjectType ArchTypes_H.apiobject_type.SchedContextObject
+                      \<longrightarrow> sc_size_bounds us"
   shows "\<lbrace>\<lambda>s. cte_wp_at' P p s \<and> valid_pspace' s \<and> pspace_no_overlap' ptr sz s\<rbrace>
   createNewCaps ty ptr n us dev
   \<lbrace>\<lambda>_. cte_wp_at' P p\<rbrace>"
   apply (wp createNewCaps_cte_wp_at')
-  apply (auto simp: cover not_0)
+  apply (auto simp: cover not_0 tysc valid_pspace'_def)
   done
 
 lemma createObjects_ret2:
@@ -3779,7 +3953,7 @@ lemma createObjects_state_refs_of'':
   "\<lbrace>\<lambda>s. n \<noteq> 0
         \<and> range_cover ptr sz (objBitsKO val + gbits) n
         \<and> P (state_refs_of' s) \<and> refs_of' val = {}
-        \<and> pspace_aligned' s \<and> pspace_distinct' s
+        \<and> pspace_aligned' s \<and> pspace_distinct' s \<and> pspace_bounded' s
         \<and> pspace_no_overlap' ptr sz s\<rbrace>
      createObjects' ptr n val gbits
    \<lbrace>\<lambda>rv s. P (state_refs_of' s)\<rbrace>"
@@ -3803,6 +3977,8 @@ crunch state_refs_of'[wp]: copyGlobalMappings "\<lambda>s. P (state_refs_of' s)"
 lemma createNewCaps_state_refs_of':
   assumes cover: "range_cover ptr sz (APIType_capBits ty us) n"
   and     not_0: "n \<noteq> 0"
+  and     tysc : "ty = APIObjectType ArchTypes_H.apiobject_type.SchedContextObject
+                         \<longrightarrow> sc_size_bounds us"
   shows
   "\<lbrace>\<lambda>s. valid_pspace' s \<and> pspace_no_overlap' ptr sz s
         \<and> P (state_refs_of' s)\<rbrace>
@@ -3816,20 +3992,21 @@ lemma createNewCaps_state_refs_of':
         apply (rename_tac apiobject_type)
         apply (case_tac apiobject_type; simp split del: if_split)
             apply (rule hoare_pre, wp, simp)
-           apply (insert cover not_0)
-           apply (wp mapM_x_wp' createObjects_state_refs_of'' threadSet_state_refs_of'
-                    | simp add: not_0 pspace_no_overlap'_def objBitsKO_def APIType_capBits_def
-                                valid_pspace'_def makeObject_tcb makeObject_endpoint objBits_def
-                                makeObject_notification archObjSize_def createObjects_def
-                                curDomain_def bit_simps
-             | intro conjI impI)+
-  done
+           apply (insert cover not_0 tysc)
+           by (wp mapM_x_wp' createObjects_state_refs_of'' threadSet_state_refs_of'
+             | simp add: not_0 pspace_no_overlap'_def objBitsKO_def APIType_capBits_def
+                         valid_pspace'_def makeObject_tcb makeObject_endpoint objBits_def
+                         makeObject_notification pageBits_def ptBits_def
+                         archObjSize_def createObjects_def curDomain_def scBits_simps
+                         pteBits_def makeObject_sc makeObject_reply pte_bits_def pt_bits_def
+                         table_size_def ptTranslationBits_def word_size_bits_def
+             | intro conjI impI )+
 
 lemma createObjects_iflive':
   "\<lbrace>\<lambda>s. if_live_then_nonz_cap' s \<and> \<not> live' val
         \<and> n \<noteq> 0
         \<and> range_cover ptr sz (objBitsKO val + gbits) n
-        \<and> pspace_aligned' s \<and> pspace_distinct' s
+        \<and> pspace_aligned' s \<and> pspace_distinct' s \<and> pspace_bounded' s
         \<and> pspace_no_overlap' ptr sz s\<rbrace>
      createObjects' ptr n val gbits
    \<lbrace>\<lambda>rv s. if_live_then_nonz_cap' s\<rbrace>"
@@ -3848,11 +4025,111 @@ lemma createObjects_iflive':
   apply (fastforce simp: ex_nonz_cap_to'_def)
   done
 
-crunch ksReadyQueues[wp]: copyGlobalMappings "\<lambda>s. P (ksReadyQueues s)"
-  (wp: updateObject_default_inv crunch_wps)
-crunch ksReadyQueuesL1[wp]: copyGlobalMappings "\<lambda>s. P (ksReadyQueuesL1Bitmap s)"
-  (wp: updateObject_default_inv crunch_wps)
-crunch ksReadyQueuesL2[wp]: copyGlobalMappings "\<lambda>s. P (ksReadyQueuesL2Bitmap s)"
+lemma createObjects_list_refs_of_replies'':
+  "\<lbrace>\<lambda>s. n \<noteq> 0
+        \<and> range_cover ptr sz (objBitsKO val + gbits) n
+        \<and> P (list_refs_of_replies' s)
+        \<and> (case val of KOReply r \<Rightarrow> replyNext_of r = None \<and> replyPrev r = None
+                     | _ \<Rightarrow> True)
+        \<and> pspace_aligned' s \<and> pspace_distinct' s \<and> pspace_bounded' s
+        \<and> pspace_no_overlap' ptr sz s\<rbrace>
+     createObjects' ptr n val gbits
+   \<lbrace>\<lambda>rv s. P (list_refs_of_replies' s)\<rbrace>" (is "\<lbrace> \<lambda>s. _ \<and> _ \<and> ?Pre s \<rbrace> _ \<lbrace>\<lambda>_. _\<rbrace>")
+proof -
+  show ?thesis
+    apply (rule hoare_grab_asm)
+    apply (rule hoare_grab_asm)
+  proof -
+    assume not_0: "\<not> n = 0"
+      and cover: "range_cover ptr sz ((objBitsKO val) + gbits) n"
+    then show
+      "\<lbrace>\<lambda>s. ?Pre s\<rbrace>
+       createObjects' ptr n val gbits
+     \<lbrace>\<lambda>rv s. P (list_refs_of_replies' s)\<rbrace>"
+    proof -
+      have shiftr_not_zero:" 1 \<le> ((of_nat n)::machine_word) << gbits"
+        using range_cover_not_zero_shift[OF not_0 cover,where gbits = gbits]
+        by (simp add:word_le_sub1)
+      note unat_of_nat_shiftl = range_cover.unat_of_nat_n_shift[OF cover,where gbits = gbits,simplified]
+      show ?thesis
+        apply (clarsimp simp: createObjects'_def unless_def alignError_def split_def)
+        apply (wp | clarsimp simp del: fun_upd_apply)+
+        apply (erule ssubst[where P = P,rotated])
+        apply (clarsimp simp: shiftL_nat data_map_insert_def[symmetric]
+                              new_cap_addrs_fold'[OF shiftr_not_zero]
+                    simp del: data_map_insert_def)
+        using range_cover.unat_of_nat_n_shift[OF cover, where gbits=gbits, simplified]
+        apply simp
+        apply (rule ext)
+        apply (rule set_eqI)
+        apply (rule iffI; clarsimp simp: map_set_def opt_map_def foldr_upd_app_if
+                                         projectKO_opt_reply list_refs_of_reply'_def
+                                  split: option.splits if_split_asm)
+         apply (cases val; fastforce)
+        apply (intro conjI impI)
+         apply clarsimp
+         apply (frule_tac x=x in retype_obj_at'_not[OF _ _ _ cover, where P=\<top>], simp+)
+          apply (simp add: semiring_normalization_rules(7))
+         apply (erule notE)
+         apply (clarsimp simp: obj_at'_def projectKOs)
+         apply (frule pspace_alignedD'; clarsimp)
+         apply (frule pspace_distinctD'; clarsimp)
+         apply (frule pspace_boundedD'; clarsimp)
+         apply (clarsimp split: kernel_object.splits)
+                 apply (rule_tac x=x2a in exI)
+                 apply (fastforce simp: projectKO_opts_defs)+
+        apply (intro allI impI)
+        apply (split kernel_object.split_asm; simp add: get_refs_def2)
+        apply (frule_tac x=x in retype_obj_at'_not[OF _ _ _ cover, where P=\<top>], simp+)
+         apply (simp add: semiring_normalization_rules(7))
+        apply (erule notE)
+        apply (clarsimp simp: obj_at'_def projectKOs)
+        apply (frule pspace_alignedD'; clarsimp)
+        apply (frule pspace_distinctD'; clarsimp)
+        apply (frule pspace_boundedD'; clarsimp)
+        apply (clarsimp split: kernel_object.splits)
+        apply (rule_tac x=x2a in exI)
+        apply (fastforce simp: projectKO_opts_defs)
+        done
+    qed
+  qed
+qed
+
+lemma createNewCaps_list_refs_of_replies':
+  assumes cover: "range_cover ptr sz (APIType_capBits ty us) n"
+  and     not_0: "n \<noteq> 0"
+  and     tysc : "ty = APIObjectType ArchTypes_H.apiobject_type.SchedContextObject
+                         \<longrightarrow> sc_size_bounds us"
+  shows
+  "\<lbrace>\<lambda>s. valid_pspace' s \<and> pspace_no_overlap' ptr sz s
+        \<and> P (list_refs_of_replies' s)\<rbrace>
+     createNewCaps ty ptr n us dev
+   \<lbrace>\<lambda>rv s. P (list_refs_of_replies' s)\<rbrace>"
+  unfolding createNewCaps_def
+  apply (clarsimp simp: RISCV64_H.toAPIType_def
+             split del: if_split)
+  apply (cases ty; simp add: createNewCaps_def Arch_createNewCaps_def
+                        split del: if_split)
+        apply (rename_tac apiobject_type)
+        apply (case_tac apiobject_type; simp split del: if_split)
+            apply (rule hoare_pre, wp, simp)
+           apply (insert cover not_0 tysc)
+           apply (wpsimp wp: mapM_x_wp' createObjects_list_refs_of_replies''
+                       simp: curDomain_def)
+           by (wpsimp wp: mapM_x_wp' createObjects_list_refs_of_replies''[simplified o_def]
+             | simp add: not_0 pspace_no_overlap'_def objBitsKO_def APIType_capBits_def
+                         valid_pspace'_def makeObject_tcb makeObject_endpoint objBits_def
+                         makeObject_notification pageBits_def ptBits_def
+                         archObjSize_def createObjects_def curDomain_def o_def scBits_simps
+                         pteBits_def makeObject_sc makeObject_reply pt_bits_def pte_bits_def
+                         word_size_bits_def table_size_def ptTranslationBits_def
+             | intro conjI impI )+
+
+crunches copyGlobalMappings
+  for ksReadyQueues[wp]: "\<lambda>s. P (ksReadyQueues s)"
+  and ksReadyQueuesL1[wp]: "\<lambda>s. P (ksReadyQueuesL1Bitmap s)"
+  and ksReadyQueuesL2[wp]: "\<lambda>s. P (ksReadyQueuesL2Bitmap s)"
+  and ksReleaseQueue[wp]: "\<lambda>s. P (ksReleaseQueue s)"
   (wp: updateObject_default_inv crunch_wps)
 
 crunch valid_idle'[wp]: copyGlobalMappings "valid_idle'"
@@ -3865,30 +4142,32 @@ crunch iflive'[wp]: copyGlobalMappings "if_live_then_nonz_cap'"
 lemma createNewCaps_iflive'[wp]:
   assumes cover: "range_cover ptr sz (APIType_capBits ty us) n"
   and     not_0: "n \<noteq> 0"
+  and     tysc : "ty = APIObjectType ArchTypes_H.apiobject_type.SchedContextObject
+                         \<longrightarrow> sc_size_bounds us"
   shows
   "\<lbrace>\<lambda>s. valid_pspace' s \<and> pspace_no_overlap' ptr sz s
         \<and> if_live_then_nonz_cap' s\<rbrace>
      createNewCaps ty ptr n us dev
    \<lbrace>\<lambda>rv s. if_live_then_nonz_cap' s\<rbrace>"
   unfolding createNewCaps_def
-  apply (insert cover)
+  apply (insert cover tysc)
   apply (clarsimp simp: toAPIType_def)
   apply (cases ty, simp_all add: createNewCaps_def Arch_createNewCaps_def
                       split del: if_split)
         apply (rename_tac apiobject_type)
         apply (case_tac apiobject_type, simp_all split del: if_split)[1]
-            apply (rule hoare_pre, wp, simp)
-           apply (wp mapM_x_wp' createObjects_iflive' threadSet_iflive'
-                  | simp add: not_0 pspace_no_overlap'_def createObjects_def
-                              valid_pspace'_def makeObject_tcb makeObject_endpoint
-                              makeObject_notification objBitsKO_def
-                              APIType_capBits_def objBits_def
-                              archObjSize_def bit_simps
-                              curDomain_def
-                         split del:if_split
-                  | simp split: if_split
-                  | fastforce)+
-  done
+              apply (rule hoare_pre, wp, simp)
+  by (wp mapM_x_wp' createObjects_iflive' threadSet_iflive'
+    | simp add: not_0 pspace_no_overlap'_def createObjects_def
+                valid_pspace'_def makeObject_tcb makeObject_endpoint
+                makeObject_notification objBitsKO_def curDomain_def scBits_simps
+                live_ntfn'_def live_sc'_def live_reply'_def makeObject_sc
+                APIType_capBits_def objBits_def pageBits_def makeObject_reply
+                archObjSize_def ptBits_def  pteBits_def pt_bits_def pte_bits_def
+                word_size_bits_def ptTranslationBits_def table_size_def
+        split del: if_split
+    | simp split: if_split
+    | fastforce)+
 
 lemma createObjects_pspace_only:
   "\<lbrakk> \<And>f s. P (ksPSpace_update f s) = P s \<rbrakk>
@@ -3902,6 +4181,10 @@ lemma createObjects'_qs[wp]:
   "\<lbrace>\<lambda>s. P (ksReadyQueues s)\<rbrace> createObjects' ptr n val gbits \<lbrace>\<lambda>rv s. P (ksReadyQueues s)\<rbrace>"
   by (rule createObjects_pspace_only, simp)
 
+lemma createObjects'_rlq[wp]:
+  "createObjects' ptr n val gbits \<lbrace>\<lambda>s. P (ksReleaseQueue s)\<rbrace>"
+  by (rule createObjects_pspace_only, simp)
+
 lemma createObjects'_qsL1[wp]:
   "\<lbrace>\<lambda>s. P (ksReadyQueuesL1Bitmap s)\<rbrace> createObjects' ptr n val gbits \<lbrace>\<lambda>rv s. P (ksReadyQueuesL1Bitmap s)\<rbrace>"
   by (rule createObjects_pspace_only, simp)
@@ -3910,17 +4193,9 @@ lemma createObjects'_qsL2[wp]:
   "\<lbrace>\<lambda>s. P (ksReadyQueuesL2Bitmap s)\<rbrace> createObjects' ptr n val gbits \<lbrace>\<lambda>rv s. P (ksReadyQueuesL2Bitmap s)\<rbrace>"
   by (rule createObjects_pspace_only, simp)
 
-(* FIXME move these 2 to TcbAcc_R *)
-lemma threadSet_qsL1[wp]:
-  "\<lbrace>\<lambda>s. P (ksReadyQueuesL1Bitmap s)\<rbrace> threadSet f t \<lbrace>\<lambda>rv s. P (ksReadyQueuesL1Bitmap s)\<rbrace>"
-  by (simp add: threadSet_def | wp updateObject_default_inv)+
-
-lemma threadSet_qsL2[wp]:
-  "\<lbrace>\<lambda>s. P (ksReadyQueuesL2Bitmap s)\<rbrace> threadSet f t \<lbrace>\<lambda>rv s. P (ksReadyQueuesL2Bitmap s)\<rbrace>"
-  by (simp add: threadSet_def | wp updateObject_default_inv)+
-
 crunches createObjects, createNewCaps
   for qs[wp]: "\<lambda>s. P (ksReadyQueues s)"
+  and rlqs[wp]: "\<lambda>s. P (ksReleaseQueue s)"
   and qsL1[wp]: "\<lambda>s. P (ksReadyQueuesL1Bitmap s)"
   and qsL2[wp]: "\<lambda>s. P (ksReadyQueuesL2Bitmap s)"
   (simp: crunch_simps wp: crunch_wps)
@@ -3977,9 +4252,8 @@ lemma copyGlobalMappings_ko_wp_at:
   apply (rule hoare_gen_asm)
   apply (simp add: copyGlobalMappings_def storePTE_def)
   apply (wp mapM_x_wp' setObject_ko_wp_at)
-      apply simp
-     apply (simp add: objBits_simps)
-    apply simp
+     apply simp
+    apply (simp add: objBits_simps)
    apply (simp cong: if_cong split del: if_split)
    apply (wp getObject_inv loadObject_default_inv | simp split del: if_split)+
    apply (clarsimp simp: obj_at'_def ko_wp_at'_def)
@@ -4022,17 +4296,18 @@ lemma mapM_x_threadSet_createNewCaps_futz:
 lemma createObjects_makeObject_not_tcbQueued:
   assumes "range_cover ptr sz (objBitsKO tcb) n"
   assumes "n \<noteq> 0" "tcb = injectKO (makeObject::tcb)"
-  shows "\<lbrace>\<lambda>s. pspace_no_overlap' ptr sz s \<and> pspace_aligned' s \<and> pspace_distinct' s\<rbrace>
+  shows "\<lbrace>\<lambda>s. pspace_no_overlap' ptr sz s \<and> pspace_aligned' s \<and> pspace_distinct' s \<and> pspace_bounded' s\<rbrace>
            createObjects ptr n tcb 0
          \<lbrace>\<lambda>rv s. \<forall>addr\<in>set rv. obj_at' (\<lambda>tcb. \<not> tcbQueued tcb \<and> tcbState tcb = Structures_H.thread_state.Inactive) addr s\<rbrace>"
   apply (rule hoare_strengthen_post[OF createObjects_ko_at_strg[where 'a=tcb]])
   using assms
-  apply (auto simp: obj_at'_def projectKO_opt_tcb objBitsKO_def objBits_def makeObject_tcb)
+  apply (auto simp: obj_at'_def projectKO_opt_tcb objBitsKO_def
+                    objBits_def makeObject_tcb)
   done
 
 lemma createObjects_ko_wp_at2:
   "\<lbrace>\<lambda>s. range_cover ptr sz (objBitsKO ko + gbits) n \<and> n \<noteq> 0
-      \<and> pspace_aligned' s \<and> pspace_distinct' s
+      \<and> pspace_aligned' s \<and> pspace_distinct' s \<and> pspace_bounded' s
       \<and> P (ko_wp_at' P' p s)
       \<and> (P' ko \<longrightarrow> P True)
       \<and> pspace_no_overlap' ptr sz s\<rbrace>
@@ -4046,13 +4321,14 @@ lemma createObjects_ko_wp_at2:
 lemma createNewCaps_ko_wp_atQ':
   "\<lbrace>(\<lambda>s. P (ko_wp_at' P' p s)
        \<and> range_cover ptr sz (APIType_capBits ty us) n \<and> n \<noteq> 0
-       \<and> pspace_aligned' s \<and> pspace_distinct' s
+       \<and> (ty = APIObjectType ArchTypes_H.apiobject_type.SchedContextObject
+               \<longrightarrow> sc_size_bounds us)
+       \<and> pspace_aligned' s \<and> pspace_distinct' s \<and> pspace_bounded' s
        \<and> pspace_no_overlap' ptr sz s)
        and K (\<forall>d (tcb_x :: tcb). \<not>tcbQueued tcb_x \<and> tcbState tcb_x = Inactive
                    \<longrightarrow> P' (injectKO (tcb_x \<lparr> tcbDomain := d \<rparr>)) = P' (injectKO tcb_x))
-       and K (\<forall>v. makeObjectKO d (Inr ty) = Some v
-                   \<longrightarrow> P' v \<longrightarrow> P True)\<rbrace>
-     createNewCaps ty ptr n us d
+       and (\<lambda>s. \<forall>v. makeObjectKO dev us (ksCurDomain s) (Inr ty) = Some v \<longrightarrow> P' v \<longrightarrow> P True)\<rbrace>
+     createNewCaps ty ptr n us dev
    \<lbrace>\<lambda>rv s. P (ko_wp_at' P' p s)\<rbrace>"
   apply (rule hoare_name_pre_state)
   apply (clarsimp simp: createNewCaps_def RISCV64_H.toAPIType_def
@@ -4062,16 +4338,16 @@ lemma createNewCaps_ko_wp_atQ':
         apply (rename_tac apiobject_type)
         apply (case_tac apiobject_type, simp_all split del: if_split)[1]
             apply (rule hoare_pre, wp, simp)
-           apply (wp mapM_x_threadSet_createNewCaps_futz
-                     mapM_x_wp'
-                     createObjects_obj_at
-                     createObjects_ko_wp_at2 createObjects_makeObject_not_tcbQueued
-                     copyGlobalMappings_ko_wp_at[where v="\<forall>pte :: pte. P' (injectKO pte)"]
+           apply ((wp mapM_x_threadSet_createNewCaps_futz
+                      mapM_x_wp'
+                      createObjects_obj_at
+                      createObjects_ko_wp_at2 createObjects_makeObject_not_tcbQueued
+                      copyGlobalMappings_ko_wp_at[where v="\<forall>pte :: pte. P' (injectKO pte)"]
                    | simp add: makeObjectKO_def objBitsKO_def archObjSize_def APIType_capBits_def
-                               objBits_def curDomain_def bit_simps
-                            split del: if_split
+                               objBits_def curDomain_def bit_simps scBits_simps
+                    split del: if_split
                    | intro conjI impI | fastforce
-                   | split if_split_asm)+
+                   | split if_split_asm)+)
   done
 
 lemmas createNewCaps_ko_wp_at'
@@ -4087,8 +4363,10 @@ lemmas createNewCaps_obj_at2 =
 lemma createNewCaps_obj_at':
   "\<lbrace>\<lambda>s. obj_at' (P :: ('a :: pspace_storable) \<Rightarrow> bool) p s
        \<and> range_cover ptr sz (APIType_capBits ty us) n \<and> n \<noteq> 0
-       \<and> pspace_aligned' s \<and> pspace_distinct' s
+       \<and> pspace_aligned' s \<and> pspace_distinct' s \<and> pspace_bounded' s
        \<and> pspace_no_overlap' ptr sz s
+       \<and> (ty = APIObjectType ArchTypes_H.apiobject_type.SchedContextObject
+                \<longrightarrow> sc_size_bounds us)
        \<and> (\<forall>tcb d. \<not>tcbQueued tcb \<and> tcbState tcb = Inactive \<longrightarrow>
             ((\<exists>obj :: 'a. injectKOS obj = KOTCB (tcb\<lparr>tcbDomain := d\<rparr>) \<and> P obj) \<longleftrightarrow>
              (\<exists>obj :: 'a. injectKOS obj = KOTCB tcb \<and> P obj)))\<rbrace>
@@ -4107,6 +4385,8 @@ lemma createNewCaps_cur:
   "\<lbrakk>range_cover ptr sz (APIType_capBits ty us) n ; n \<noteq> 0\<rbrakk> \<Longrightarrow>
    \<lbrace>\<lambda>s. valid_pspace' s \<and>
         pspace_no_overlap' ptr sz s \<and>
+        (ty = APIObjectType ArchTypes_H.apiobject_type.SchedContextObject
+                \<longrightarrow> sc_size_bounds us) \<and>
         cur_tcb' s\<rbrace>
       createNewCaps ty ptr n us d
    \<lbrace>\<lambda>rv. cur_tcb'\<rbrace>"
@@ -4125,6 +4405,8 @@ lemma createNewCaps_ifunsafe':
   "\<lbrace>\<lambda>s. valid_pspace' s \<and>
         pspace_no_overlap' ptr sz s \<and>
         range_cover ptr sz (APIType_capBits ty us) n \<and> n \<noteq> 0 \<and>
+        (ty = APIObjectType ArchTypes_H.apiobject_type.SchedContextObject
+               \<longrightarrow> sc_size_bounds us) \<and>
         if_unsafe_then_cap' s\<rbrace>
       createNewCaps ty ptr n us d
    \<lbrace>\<lambda>rv s. if_unsafe_then_cap' s\<rbrace>"
@@ -4136,7 +4418,7 @@ lemma createNewCaps_ifunsafe':
              createNewCaps_cte_wp_at2 hoare_vcg_ex_lift)
   apply (simp add: makeObject_cte pspace_no_overlap'_def
                    valid_pspace'_def)
-  apply auto
+  apply (auto simp: scBits_simps)
   done
 
 lemma createObjects_nosch'[wp]:
@@ -4145,12 +4427,10 @@ lemma createObjects_nosch'[wp]:
    \<lbrace>\<lambda>rv s. P (ksSchedulerAction s)\<rbrace>"
   by (rule createObjects_pspace_only, simp)
 
-crunch nosch[wp]: copyGlobalMappings "\<lambda>s. P (ksSchedulerAction s)"
-  (wp: setObject_ksPSpace_only updateObject_default_inv mapM_x_wp')
-crunches createObjects, createNewCaps
+crunches copyGlobalMappings, createObjects, createNewCaps
   for nosch[wp]: "\<lambda>s. P (ksSchedulerAction s)"
   and it[wp]: "\<lambda>s. P (ksIdleThread s)"
-  (simp: crunch_simps wp: crunch_wps)
+  (wp: setObject_ksPSpace_only updateObject_default_inv mapM_x_wp')
 
 lemma createObjects_idle':
   "\<lbrace>valid_idle' and valid_pspace' and pspace_no_overlap' ptr sz
@@ -4178,6 +4458,8 @@ lemma createObjects_idle':
 
 lemma createNewCaps_idle'[wp]:
   "\<lbrace>valid_idle' and valid_pspace' and pspace_no_overlap' ptr sz
+       and K (ty = APIObjectType ArchTypes_H.apiobject_type.SchedContextObject
+                   \<longrightarrow> sc_size_bounds us)
        and K (range_cover ptr sz (APIType_capBits ty us) n \<and> n \<noteq> 0)\<rbrace>
    createNewCaps ty ptr n us d
    \<lbrace>\<lambda>rv. valid_idle'\<rbrace>"
@@ -4188,18 +4470,12 @@ lemma createNewCaps_idle'[wp]:
                       split del: if_split)
          apply (rename_tac apiobject_type)
          apply (case_tac apiobject_type, simp_all split del: if_split)[1]
-             apply (wp, simp)
-           including no_pre
-           apply (wp mapM_x_wp'
-                     createObjects_idle'
-                     threadSet_idle'
-                   | simp add: projectKO_opt_tcb projectKO_opt_cte
-                               makeObject_cte makeObject_tcb archObjSize_def
-                               tcb_cte_cases_def objBitsKO_def APIType_capBits_def
-                               objBits_def createObjects_def bit_simps cteSizeBits_def
-                   | intro conjI impI
-                   | fastforce simp: curDomain_def)+
-  done
+  by (wpsimp wp: createObjects_idle'[where sz=sz] mapM_x_wp' split_del: if_split
+           simp:  curDomain_def APIType_capBits_def createObjects_def
+    | simp add: tcb_cte_cases_def projectKO_opt_tcb projectKO_opt_cte makeObject_tcb makeObject_cte
+                ptBits_def pteBits_def pageBits_def objBits_simps'
+                pt_bits_def pte_bits_def word_size_bits_def table_size_def ptTranslationBits_def
+                scBits_simps)+
 
 crunch ksArch[wp]: createNewCaps "\<lambda>s. P (ksArchState s)"
   (simp: crunch_simps unless_def wp: crunch_wps)
@@ -4208,8 +4484,10 @@ crunch gsMaxObjectSize[wp]: createNewCaps "\<lambda>s. P (gsMaxObjectSize s)"
 
 lemma createNewCaps_global_refs':
   "\<lbrace>\<lambda>s. range_cover ptr sz (APIType_capBits ty us) n \<and> n \<noteq> 0
-       \<and> pspace_aligned' s \<and> pspace_distinct' s
+       \<and> pspace_aligned' s \<and> pspace_distinct' s \<and> pspace_bounded' s
        \<and> pspace_no_overlap' ptr sz s \<and> valid_global_refs' s
+       \<and> (ty = APIObjectType ArchTypes_H.apiobject_type.SchedContextObject
+                \<longrightarrow> sc_size_bounds us)
        \<and> 0 < gsMaxObjectSize s\<rbrace>
      createNewCaps ty ptr n us d
    \<lbrace>\<lambda>rv. valid_global_refs'\<rbrace>"
@@ -4225,8 +4503,7 @@ lemma createNewCaps_global_refs':
    apply (rule hoare_use_eq [where f=irq_node', OF createNewCaps_ksInterrupt])
    apply (rule hoare_use_eq [where f=gsMaxObjectSize], wp)
    apply (wp hoare_vcg_all_lift createNewCaps_cte_wp_at2[where sz=sz])
-  apply (clarsimp simp: cte_wp_at_ctes_of global_refs'_def
-                        makeObject_cte)
+  apply (clarsimp simp: cte_wp_at_ctes_of global_refs'_def sc_size_bounds_def makeObject_cte)
   apply (auto simp: linorder_not_less ball_ran_eq)
   done
 
@@ -4237,7 +4514,9 @@ lemma koTypeOf_eq_UserDataT:
 
 lemma createNewCaps_valid_arch_state:
   "\<lbrace>(\<lambda>s. valid_arch_state' s \<and> valid_pspace' s \<and> pspace_no_overlap' ptr sz s
-        \<and> (tp = APIObjectType ArchTypes_H.CapTableObject \<longrightarrow> us > 0))
+        \<and> (tp = APIObjectType ArchTypes_H.CapTableObject \<longrightarrow> us > 0)
+        \<and> (ty = APIObjectType ArchTypes_H.apiobject_type.SchedContextObject
+                \<longrightarrow> sc_size_bounds us))
        and K (range_cover ptr sz (APIType_capBits ty us) n \<and> n \<noteq> 0)\<rbrace>
      createNewCaps ty ptr n us d
    \<lbrace>\<lambda>rv. valid_arch_state'\<rbrace>"
@@ -4278,7 +4557,9 @@ lemma valid_irq_handlers_cte_wp_at_form':
 
 lemma createNewCaps_irq_handlers':
   "\<lbrace>valid_irq_handlers' and pspace_no_overlap' ptr sz
-       and pspace_aligned' and pspace_distinct'
+       and pspace_aligned' and pspace_distinct' and pspace_bounded'
+       and K (ty = APIObjectType ArchTypes_H.apiobject_type.SchedContextObject
+                   \<longrightarrow> sc_size_bounds us)
        and K (range_cover ptr sz (APIType_capBits ty us) n \<and> n \<noteq> 0)\<rbrace>
      createNewCaps ty ptr n us d
    \<lbrace>\<lambda>rv. valid_irq_handlers'\<rbrace>"
@@ -4286,7 +4567,7 @@ lemma createNewCaps_irq_handlers':
    apply (wp hoare_vcg_all_lift hoare_vcg_disj_lift
              createNewCaps_cte_wp_at2)
   apply (clarsimp simp: makeObject_cte)
-  apply auto
+  apply (auto simp: sc_size_bounds_def)
   done
 
 lemma createObjects'_irq_states' [wp]:
@@ -4304,7 +4585,9 @@ crunch ksMachine[wp]: createObjects "\<lambda>s. P (ksMachineState s)"
 
 lemma createNewCaps_valid_queues':
   "\<lbrace>valid_queues' and pspace_no_overlap' ptr sz
-       and pspace_aligned' and pspace_distinct'
+       and pspace_aligned' and pspace_distinct' and pspace_bounded'
+       and K (ty = APIObjectType ArchTypes_H.apiobject_type.SchedContextObject
+                \<longrightarrow> sc_size_bounds us)
        and K (range_cover ptr sz (APIType_capBits ty us) n \<and> n \<noteq> 0)\<rbrace>
      createNewCaps ty ptr n us d
    \<lbrace>\<lambda>rv. valid_queues'\<rbrace>"
@@ -4320,12 +4603,66 @@ lemma createNewCaps_valid_queues':
 
 lemma createNewCaps_valid_queues:
   "\<lbrace>valid_queues and pspace_no_overlap' ptr sz
-       and pspace_aligned' and pspace_distinct'
+       and pspace_aligned' and pspace_distinct' and pspace_bounded'
+       and K (ty = APIObjectType ArchTypes_H.apiobject_type.SchedContextObject
+                \<longrightarrow> sc_size_bounds us)
        and K (range_cover ptr sz (APIType_capBits ty us) n \<and> n \<noteq> 0)\<rbrace>
      createNewCaps ty ptr n us d
    \<lbrace>\<lambda>rv. valid_queues\<rbrace>"
   apply (rule hoare_gen_asm)
   apply (wp valid_queues_lift_asm createNewCaps_obj_at2[where sz=sz])
+       apply (clarsimp simp: projectKO_opts_defs)
+       apply (simp add: inQ_def)
+      apply (wp createNewCaps_pred_tcb_at'[where sz=sz] | simp)+
+  done
+
+lemma valid_release_queue_lift_asm':
+  assumes tat: "\<And>t. \<lbrace>\<lambda>s. \<not> obj_at' tcbInReleaseQueue t s \<and> Q s\<rbrace> f \<lbrace>\<lambda>_ s. \<not> obj_at' tcbInReleaseQueue t s\<rbrace>"
+  and     prq: "\<And>P. \<lbrace>\<lambda>s. P (ksReleaseQueue s)\<rbrace> f \<lbrace>\<lambda>_ s. P (ksReleaseQueue s)\<rbrace>"
+  shows   "\<lbrace>\<lambda>s. valid_release_queue' s \<and> Q s\<rbrace> f \<lbrace>\<lambda>_. valid_release_queue'\<rbrace>"
+  apply (simp only: valid_release_queue'_def imp_conv_disj)
+  apply (wp hoare_vcg_all_lift hoare_vcg_disj_lift
+            tat prq)
+  apply simp
+  done
+
+lemma valid_release_queue_lift_asm:
+  assumes tat: "\<And>tcb. \<lbrace>obj_at' tcbInReleaseQueue tcb and Q \<rbrace> f \<lbrace>\<lambda>_. obj_at' tcbInReleaseQueue tcb\<rbrace>"
+  and     prq: "\<And>P. \<lbrace>\<lambda>s. P (ksReleaseQueue s) \<rbrace> f \<lbrace>\<lambda>_ s. P (ksReleaseQueue s)\<rbrace>"
+  shows   "\<lbrace>Invariants_H.valid_release_queue and Q\<rbrace> f \<lbrace>\<lambda>_. Invariants_H.valid_release_queue\<rbrace>"
+  apply (simp only: valid_release_queue_def imp_conv_disj)
+  apply (wp hoare_vcg_all_lift hoare_vcg_disj_lift
+            tat prq)
+  apply simp
+  done
+
+lemma createNewCaps_valid_release_queue':
+  "\<lbrace>valid_release_queue' and pspace_no_overlap' ptr sz
+       and pspace_aligned' and pspace_distinct' and pspace_bounded'
+       and K (ty = APIObjectType ArchTypes_H.apiobject_type.SchedContextObject
+                \<longrightarrow> sc_size_bounds us)
+       and K (range_cover ptr sz (APIType_capBits ty us) n \<and> n \<noteq> 0)\<rbrace>
+     createNewCaps ty ptr n us d
+   \<lbrace>\<lambda>rv. valid_release_queue'\<rbrace>"
+  apply (wp valid_release_queue_lift_asm' [OF createNewCaps_obj_at2])
+  apply (clarsimp simp: projectKOs)
+  apply (simp add: makeObjectKO_def
+            split: object_type.split_asm
+                   apiobject_type.split_asm)
+  apply (auto simp: makeObject_tcb
+             split: object_type.splits apiobject_type.splits)
+  done
+
+lemma createNewCaps_valid_release_queue:
+  "\<lbrace>valid_release_queue and pspace_no_overlap' ptr sz
+       and pspace_aligned' and pspace_distinct' and pspace_bounded'
+       and K (ty = APIObjectType ArchTypes_H.apiobject_type.SchedContextObject
+                \<longrightarrow> sc_size_bounds us)
+       and K (range_cover ptr sz (APIType_capBits ty us) n \<and> n \<noteq> 0)\<rbrace>
+     createNewCaps ty ptr n us d
+   \<lbrace>\<lambda>rv. valid_release_queue\<rbrace>"
+  apply (rule hoare_gen_asm)
+  apply (wp valid_release_queue_lift_asm createNewCaps_obj_at2[where sz=sz])
        apply (clarsimp simp: projectKO_opts_defs)
        apply (simp add: inQ_def)
       apply (wp createNewCaps_pred_tcb_at'[where sz=sz] | simp)+
@@ -4345,25 +4682,36 @@ lemma createNewCaps_valid_pspace:
   and      sz_limit: "sz \<le> maxUntypedSizeBits"
   and      ptr_cn: "canonical_address (ptr && ~~ mask sz)"
   and      ptr_km: "ptr && ~~ mask sz \<in> kernel_mappings"
-  shows "\<lbrace>\<lambda>s. pspace_no_overlap' ptr sz s \<and> valid_pspace' s
-  \<and> caps_no_overlap'' ptr sz s \<and> ptr \<noteq> 0 \<and> caps_overlap_reserved' {ptr..ptr + of_nat n * 2^(APIType_capBits ty us) - 1} s \<and> ksCurDomain s \<le> maxDomain\<rbrace>
-  createNewCaps ty ptr n us dev \<lbrace>\<lambda>r. valid_pspace'\<rbrace>"
+  and       tysc: "ty = APIObjectType ArchTypes_H.apiobject_type.SchedContextObject
+                     \<longrightarrow> sc_size_bounds us"
+  shows
+  "\<lbrace>\<lambda>s. pspace_no_overlap' ptr sz s \<and> valid_pspace' s
+     \<and> caps_no_overlap'' ptr sz s \<and> ptr \<noteq> 0 \<and> caps_overlap_reserved' {ptr..ptr + of_nat n * 2^(APIType_capBits ty us) - 1} s
+     \<and> ksCurDomain s \<le> maxDomain\<rbrace>
+   createNewCaps ty ptr n us dev
+   \<lbrace>\<lambda>r. valid_pspace'\<rbrace>"
   unfolding createNewCaps_def Arch_createNewCaps_def
-  using valid_obj_makeObject_rules ptr_cn sz_limit ptr_km
+  using valid_obj_makeObject_rules
   apply (clarsimp simp: RISCV64_H.toAPIType_def
              split del: if_split cong: option.case_cong)
   apply (cases ty, simp_all split del: if_split)
         apply (rename_tac apiobject_type)
         apply (case_tac apiobject_type, simp_all split del: if_split)
-            apply (rule hoare_pre, wp, clarsimp)
-           apply (insert cover)
-           apply (wp createObjects_valid_pspace_untyped' [OF _ not_0 , where ty="Inr ty" and sz = sz]
-                     mapM_x_threadSet_valid_pspace mapM_x_wp'
-                 | simp add: makeObjectKO_def APIType_capBits_def
-                             objBits_simps not_0 createObjects_def curDomain_def bit_simps
-                 | intro conjI impI
-                 | simp add: power_add field_simps)+
-  done
+              apply (rule hoare_pre, wp, clarsimp)
+             apply (insert cover tysc sz_limit ptr_cn ptr_km)
+             (* for TCBObject, we need to know a bit more about tcbDomain *)
+             apply (simp add: curDomain_def)
+             apply (rule hoare_seq_ext[OF _ gets_sp])
+             apply (clarsimp simp: createObjects_def)
+             apply (rule hoare_assume_pre)
+  by (wpsimp wp: createObjects_valid_pspace_untyped'[of dev us _ "Inr ty", where ptr=ptr]
+                 mapM_x_wp'
+          split_del: if_split
+          simp: createObjects_def makeObjectKO_def objBits_def objBitsKO_def scBits_simps
+                power_add not_0 APIType_capBits_def field_simps pageBits_def
+                archObjSize_def ptBits_def pteBits_def scBits_simps
+                ptTranslationBits_def pt_bits_def pte_bits_def word_size_bits_def table_size_def
+    | simp)+
 
 lemma copyGlobalMappings_inv[wp]:
   "\<lbrace>\<lambda>s. P (ksMachineState s)\<rbrace>
@@ -4382,9 +4730,20 @@ lemma doMachineOp_return_foo:
   apply clarsimp
   done
 
+lemma doMachineOp_mapM_x_wp:
+  assumes empty_fail:"\<And>x. empty_fail (f x)"
+  assumes valid: "\<And>z. \<lbrace>P\<rbrace> doMachineOp (f z) \<lbrace>\<lambda>y. P\<rbrace>"
+  shows "\<lbrace>P\<rbrace> doMachineOp (mapM_x f xs) \<lbrace>\<lambda>y. P\<rbrace>"
+  apply (clarsimp simp: mapM_x_mapM doMachineOp_return_foo)
+  apply (subst doMachineOp_mapM)
+  apply (wp valid empty_fail mapM_wp' | simp)+
+  done
+
 lemma createNewCaps_vms:
-  "\<lbrace>pspace_aligned' and pspace_distinct' and pspace_no_overlap' ptr sz and
+  "\<lbrace>pspace_aligned' and pspace_distinct' and pspace_bounded' and pspace_no_overlap' ptr sz and
     K (range_cover ptr sz (APIType_capBits ty us) n \<and> 0 < n) and
+    K (ty = APIObjectType ArchTypes_H.apiobject_type.SchedContextObject
+                \<longrightarrow> sc_size_bounds us) and
     valid_machine_state'\<rbrace>
    createNewCaps ty ptr n us dev
    \<lbrace>\<lambda>archCaps. valid_machine_state'\<rbrace>"
@@ -4398,14 +4757,15 @@ lemma createNewCaps_vms:
            hoare_vcg_all_lift
            doMachineOp_ko_wp_at' createObjects_orig_ko_wp_at2'[where sz = sz]
            hoare_vcg_all_lift
-           dmo_lift' mapM_x_wp' copyGlobalMappings_ko_wp_at threadSet_ko_wp_at2'
+           doMachineOp_mapM_x_wp dmo_lift' mapM_x_wp' copyGlobalMappings_ko_wp_at threadSet_ko_wp_at2'
          | clarsimp simp: createObjects_def Arch_createNewCaps_def curDomain_def Let_def
+                          pteBits_def
                split del: if_split
          | assumption)+
   apply (case_tac ty)
-   apply (auto simp: APIType_capBits_def objBits_simps
-                     toAPIType_def object_type.splits bit_simps)
-  done
+  by (auto simp: APIType_capBits_def objBits_simps pageBits_def ptBits_def
+                 RISCV64_H.toAPIType_def object_type.splits pteBits_def scBits_simps
+                 pte_bits_def pt_bits_def word_size_bits_def ptTranslationBits_def table_size_def)
 
 lemma createObjects_pspace_domain_valid':
   "\<lbrace>\<lambda>s. range_cover ptr sz (objBitsKO val + gbits) n \<and> n \<noteq> 0
@@ -4448,7 +4808,9 @@ crunch pspace_domain_valid[wp]: copyGlobalMappings "pspace_domain_valid"
 lemma createNewCaps_pspace_domain_valid[wp]:
   "\<lbrace>pspace_domain_valid and K ({ptr .. (ptr && ~~ mask sz) + 2 ^ sz - 1}
             \<inter> kernel_data_refs = {}
-        \<and> range_cover ptr sz (APIType_capBits ty us) n \<and> 0 < n)\<rbrace>
+        \<and> range_cover ptr sz (APIType_capBits ty us) n \<and> 0 < n)
+       and K (ty = APIObjectType ArchTypes_H.apiobject_type.SchedContextObject
+                \<longrightarrow> sc_size_bounds us)\<rbrace>
     createNewCaps ty ptr n us dev
    \<lbrace>\<lambda>rv. pspace_domain_valid\<rbrace>"
   apply (simp add: createNewCaps_def)
@@ -4459,7 +4821,7 @@ lemma createNewCaps_pspace_domain_valid[wp]:
                      split del: if_split)+
   apply (simp add: RISCV64_H.toAPIType_def
             split: object_type.splits)
-  apply (auto simp: objBits_simps APIType_capBits_def bit_simps)
+  apply (auto simp: objBits_simps APIType_capBits_def bit_simps scBits_simps)
   done
 
 (* FIXME: move *)
@@ -4490,11 +4852,14 @@ proof -
 qed
 
 lemma createNewCaps_ct_idle_or_in_cur_domain':
-  "\<lbrace>ct_idle_or_in_cur_domain' and pspace_aligned' and pspace_distinct' and pspace_no_overlap' ptr sz and ct_active' and K (range_cover ptr sz (APIType_capBits ty us) n \<and> 0 < n) \<rbrace>
+  "\<lbrace>ct_idle_or_in_cur_domain' and pspace_aligned' and pspace_distinct' and pspace_bounded'
+    and pspace_no_overlap' ptr sz
+    and K (ty = APIObjectType ArchTypes_H.apiobject_type.SchedContextObject
+                \<longrightarrow> sc_size_bounds us)
+    and ct_active' and K (range_cover ptr sz (APIType_capBits ty us) n \<and> 0 < n) \<rbrace>
     createNewCaps ty ptr n us dev
    \<lbrace>\<lambda>rv. ct_idle_or_in_cur_domain'\<rbrace>"
-  apply (wp ct_idle_or_in_cur_domain'_lift_futz createNewCaps_obj_at'[where sz=sz] | simp)+
-  done
+  by (wp ct_idle_or_in_cur_domain'_lift_futz createNewCaps_obj_at'[where sz=sz] | simp)+
 
 lemma sch_act_wf_lift_asm_futz:
   assumes tcb: "\<And>P t. \<lbrace>st_tcb_at' P t and Q \<rbrace> f \<lbrace>\<lambda>rv. st_tcb_at' P t\<rbrace>"
@@ -4526,7 +4891,11 @@ lemma sch_act_wf_lift_asm_futz:
   done
 
 lemma createNewCaps_sch_act_wf:
-  "\<lbrace>(\<lambda>s. sch_act_wf (ksSchedulerAction s) s) and pspace_aligned' and pspace_distinct' and pspace_no_overlap' ptr sz and K (range_cover ptr sz (APIType_capBits ty us) n \<and> 0 < n)\<rbrace>
+  "\<lbrace>(\<lambda>s. sch_act_wf (ksSchedulerAction s) s) and pspace_aligned' and pspace_distinct'
+       and pspace_bounded' and pspace_no_overlap' ptr sz
+       and K (ty = APIObjectType ArchTypes_H.apiobject_type.SchedContextObject
+                \<longrightarrow> sc_size_bounds us)
+       and K (range_cover ptr sz (APIType_capBits ty us) n \<and> 0 < n)\<rbrace>
      createNewCaps ty ptr n us dev
    \<lbrace>\<lambda>_ s. sch_act_wf (ksSchedulerAction s) s\<rbrace>"
   apply (wp sch_act_wf_lift_asm_futz
@@ -4559,38 +4928,45 @@ crunch ksDomScheduleIdx[wp]: createNewCaps "\<lambda>s. P (ksDomScheduleIdx s)"
   (wp: mapM_x_wp' simp: crunch_simps)
 
 lemma createObjects_null_filter':
-  "\<lbrace>\<lambda>s. P (null_filter' (ctes_of s)) \<and> makeObjectKO dev ty = Some val \<and>
+  "\<lbrace>\<lambda>s. P (null_filter' (ctes_of s)) \<and> makeObjectKO dev us d ty = Some val \<and>
         range_cover ptr sz (objBitsKO val + gbits) n \<and> n \<noteq> 0 \<and>
-        pspace_aligned' s \<and> pspace_distinct' s \<and> pspace_no_overlap' ptr sz s\<rbrace>
+        pspace_aligned' s \<and> pspace_distinct' s \<and> pspace_bounded' s \<and> pspace_no_overlap' ptr sz s\<rbrace>
    createObjects' ptr n val gbits
    \<lbrace>\<lambda>addrs a. P (null_filter' (ctes_of a))\<rbrace>"
-   apply (clarsimp simp: createObjects'_def split_def)
-   apply (wp hoare_unless_wp|wpc
-          | clarsimp simp: alignError_def split del: if_split simp del:fun_upd_apply)+
-   apply (subst new_cap_addrs_fold')
-     apply (simp add:unat_1_0 unat_gt_0)
-     apply (rule range_cover_not_zero_shift)
+  apply (clarsimp simp: createObjects'_def split_def)
+  apply (wp hoare_unless_wp|wpc
+         | clarsimp simp: alignError_def split del: if_split simp del:fun_upd_apply)+
+  apply (subst new_cap_addrs_fold')
+   apply (simp add:unat_1_0 unat_gt_0)
+   apply (rule range_cover_not_zero_shift)
      apply fastforce+
-   apply (subst new_cap_addrs_fold')
-    apply (simp add:unat_1_0 unat_gt_0)
-    apply (rule range_cover_not_zero_shift)
-      apply simp
-     apply assumption
-    apply simp
-   apply (subst data_map_insert_def[symmetric])+
-   apply (frule(2) retype_aligned_distinct'[where ko = val])
-    apply (erule range_cover_rel)
-     apply simp+
-   apply (frule(2) retype_aligned_distinct'(2)[where ko = val])
-    apply (erule range_cover_rel)
-     apply simp+
-   apply (frule null_filter_ctes_retype
-     [where addrs = "(new_cap_addrs (unat (((of_nat n)::machine_word) << gbits)) ptr val)"])
-          apply assumption+
-     apply (clarsimp simp:field_simps foldr_upd_app_if[folded data_map_insert_def] shiftl_t2n range_cover.unat_of_nat_shift)+
+  apply (subst new_cap_addrs_fold')
+   apply (simp add:unat_1_0 unat_gt_0)
+   apply (rule range_cover_not_zero_shift)
+     apply simp
+    apply assumption
+   apply simp
+  apply (subst data_map_insert_def[symmetric])+
+  apply (frule (3) retype_aligned_distinct'[where ko = val])
+   apply (erule range_cover_rel)
+    apply simp+
+  apply (frule (3) retype_aligned_distinct'(2)[where ko = val])
+   apply (erule range_cover_rel)
+    apply simp+
+  apply (frule (3) retype_aligned_distinct'(3)[where ko = val])
+   apply (erule range_cover_rel)
+    apply simp+
+  apply (frule null_filter_ctes_retype[where addrs =
+                                       "new_cap_addrs (unat ((of_nat n::machine_word) << gbits)) ptr val"])
+        apply assumption+
+       apply (prop_tac "objBitsKO val < word_bits")
+        apply (clarsimp simp: range_cover_def word_bits_def)
+      apply (clarsimp simp: field_simps foldr_upd_app_if[folded data_map_insert_def] shiftl_t2n
+                            range_cover.unat_of_nat_shift)+
     apply (rule new_cap_addrs_aligned[THEN bspec])
-    apply (erule range_cover.aligned[OF range_cover_rel])
-     apply simp+
+     apply (erule range_cover.aligned[OF range_cover_rel])
+      apply simp+
+    apply (clarsimp simp: range_cover_def word_bits_def)
    apply (clarsimp simp:shiftl_t2n field_simps range_cover.unat_of_nat_shift)
    apply (drule subsetD[OF new_cap_addrs_subset,rotated])
     apply (erule range_cover_rel)
@@ -4603,15 +4979,17 @@ lemma createObjects_null_filter':
     apply (drule(1) pspace_alignedD')
     apply (clarsimp)
     apply (erule is_aligned_no_overflow)
-    apply (simp del:atLeastAtMost_iff atLeastatMost_subset_iff atLeastLessThan_iff
-        Int_atLeastAtMost atLeastatMost_empty_iff add:Int_ac ptr_add_def p_assoc_help)
+   apply (simp del: atLeastAtMost_simps
+               add: Int_ac ptr_add_def p_assoc_help)
   apply (simp add:field_simps foldr_upd_app_if[folded data_map_insert_def] shiftl_t2n)
   apply auto
   done
 
 lemma createNewCaps_null_filter':
   "\<lbrace>(\<lambda>s. P (null_filter' (ctes_of s)))
-      and pspace_aligned' and pspace_distinct' and pspace_no_overlap' ptr sz
+      and pspace_aligned' and pspace_distinct' and pspace_bounded' and pspace_no_overlap' ptr sz
+      and K (ty = APIObjectType ArchTypes_H.apiobject_type.SchedContextObject
+                \<longrightarrow> sc_size_bounds us)
       and K (range_cover ptr sz (APIType_capBits ty us) n \<and> n \<noteq> 0) \<rbrace>
      createNewCaps ty ptr n us dev
    \<lbrace>\<lambda>_ s. P (null_filter' (ctes_of s))\<rbrace>"
@@ -4623,14 +5001,15 @@ lemma createNewCaps_null_filter':
           apply (rename_tac apiobject_type)
           apply (case_tac apiobject_type, simp_all split del: if_split)
               apply (rule hoare_pre, wp,simp)
-             apply (simp add: createObjects_def makeObjectKO_def APIType_capBits_def objBits_def
-                              archObjSize_def curDomain_def objBits_if_dev bit_simps
-                       split del: if_split
-                    | wp createObjects_null_filter'[where ty = "Inr ty" and sz = sz and dev=dev]
-                         copyGlobalMappings_ctes_of threadSet_ctes_of mapM_x_wp'
-                    | simp add: objBits_simps
-                    | fastforce)+
-  done
+             by (simp add: createObjects_def makeObjectKO_def scBits_simps
+                           APIType_capBits_def objBits_def pageBits_def
+                           archObjSize_def ptBits_def curDomain_def objBits_if_dev
+                    split del: if_split
+                | wp createObjects_null_filter'[where ty = "Inr ty" and sz = sz and dev=dev]
+                     copyGlobalMappings_ctes_of threadSet_ctes_of mapM_x_wp'
+                | simp add: objBits_simps pteBits_def pt_bits_def pte_bits_def
+                            word_size_bits_def ptTranslationBits_def table_size_def
+                | fastforce)+
 
 crunch gsUntypedZeroRanges[wp]: createNewCaps "\<lambda>s. P (gsUntypedZeroRanges s)"
   (wp: mapM_x_wp' simp: crunch_simps)
@@ -4651,7 +5030,9 @@ lemma untyped_ranges_zero_inv_null_filter_cteCaps_of:
 
 lemma createNewCaps_urz:
   "\<lbrace>untyped_ranges_zero'
-      and pspace_aligned' and pspace_distinct' and pspace_no_overlap' ptr sz
+      and pspace_aligned' and pspace_distinct' and pspace_bounded' and pspace_no_overlap' ptr sz
+      and K (ty = APIObjectType ArchTypes_H.apiobject_type.SchedContextObject
+                \<longrightarrow> sc_size_bounds us)
       and K (range_cover ptr sz (APIType_capBits ty us) n \<and> n \<noteq> 0) \<rbrace>
    createNewCaps ty ptr n us dev
    \<lbrace>\<lambda>archCaps. untyped_ranges_zero'\<rbrace>"
@@ -4670,6 +5051,7 @@ lemma createNewCaps_invs':
         \<and> (ty = APIObjectType ArchTypes_H.CapTableObject \<longrightarrow> us > 0)
         \<and> gsMaxObjectSize s > 0)
        and K (range_cover ptr sz (APIType_capBits ty us) n \<and> n \<noteq> 0
+              \<and> (ty = APIObjectType ArchTypes_H.SchedContextObject \<longrightarrow> sc_size_bounds us)
               \<and> sz \<le> maxUntypedSizeBits \<and> canonical_address (ptr && ~~ mask sz)
               \<and> ptr && ~~ mask sz \<in> kernel_mappings)\<rbrace>
      createNewCaps ty ptr n us dev
@@ -4678,29 +5060,16 @@ lemma createNewCaps_invs':
 proof (rule hoare_gen_asm, elim conjE)
   assume cover: "range_cover ptr sz (APIType_capBits ty us) n"
     and  not_0: "n \<noteq> 0"
+    and  tysc: "ty = APIObjectType ArchTypes_H.SchedContextObject \<longrightarrow> sc_size_bounds us"
     and  sz_limit: "sz \<le> maxUntypedSizeBits"
     and  ptr_cn: "canonical_address (ptr && ~~ mask sz)"
     and  ptr_km: "ptr && ~~ mask sz \<in> kernel_mappings"
-  have cnc_ct_not_inQ:
-    "\<lbrace>ct_not_inQ and valid_pspace' and pspace_no_overlap' ptr sz\<rbrace>
-     createNewCaps ty ptr n us dev \<lbrace>\<lambda>_. ct_not_inQ\<rbrace>"
-    unfolding ct_not_inQ_def
-    apply (rule_tac Q="\<lambda>s. ksSchedulerAction s = ResumeCurrentThread
-                             \<longrightarrow> (obj_at' (Not \<circ> tcbQueued) (ksCurThread s) s
-                                  \<and> valid_pspace' s \<and> pspace_no_overlap' ptr sz s)"
-                    in hoare_pre_imp, clarsimp)
-    apply (rule hoare_convert_imp [OF createNewCaps_nosch])
-    apply (rule hoare_weaken_pre)
-     apply (wps createNewCaps_ct)
-     apply (wp createNewCaps_obj_at')
-    using cover not_0
-    apply (fastforce simp: valid_pspace'_def)
-    done
   show "\<lbrace>?P\<rbrace>
      createNewCaps ty ptr n us dev
    \<lbrace>\<lambda>rv. invs'\<rbrace>"
-  apply (simp add: invs'_def valid_state'_def
-                   pointerInUserData_def typ_at'_def)
+  apply -
+  apply (simp add: invs'_def valid_dom_schedule'_def
+                   pointerInUserData_def typ_at'_def sc_size_bounds_def)
     apply (rule hoare_pre)
      apply (wp createNewCaps_valid_pspace [OF not_0 cover sz_limit ptr_cn ptr_km]
                createNewCaps_state_refs_of' [OF cover not_0 ]
@@ -4714,16 +5083,20 @@ proof (rule hoare_gen_asm, elim conjE)
                createNewCaps_irq_handlers' createNewCaps_vms
                createNewCaps_valid_queues
                createNewCaps_valid_queues'
-               createNewCaps_pred_tcb_at' cnc_ct_not_inQ
+               createNewCaps_valid_release_queue
+               createNewCaps_valid_release_queue'
+               createNewCaps_valid_queues
+               createNewCaps_valid_queues'
+               createNewCaps_pred_tcb_at'
                createNewCaps_ct_idle_or_in_cur_domain'
                createNewCaps_sch_act_wf
                createNewCaps_urz[where sz=sz]
-           | simp)+
+               createNewCaps_list_refs_of_replies' [OF cover not_0]
+           | simp add: tysc)+
   using not_0
   apply (clarsimp simp: valid_pspace'_def)
   using cover
-  apply (intro conjI)
-   apply simp_all
+  apply (intro conjI; simp)
   done
 qed
 
@@ -4756,7 +5129,7 @@ lemma createObjects_obj_ranges':
 
 lemma createObjects_pred_tcb_at':
   "\<lbrace>pred_tcb_at' proj P t and K (range_cover ptr sz (objBitsKO val + gbits) n \<and> n \<noteq> 0)
-     and pspace_aligned' and pspace_distinct' and pspace_no_overlap' ptr sz\<rbrace>
+     and pspace_aligned' and pspace_distinct' and pspace_bounded' and pspace_no_overlap' ptr sz\<rbrace>
   createObjects ptr n val gbits \<lbrace>\<lambda>rv. pred_tcb_at' proj P t\<rbrace>"
   apply (simp add: pred_tcb_at'_def createObjects_def)
   apply (wp createObjects_orig_obj_at')
@@ -4765,7 +5138,7 @@ lemma createObjects_pred_tcb_at':
 
 lemma createObjects_ex_cte_cap_to [wp]:
   "\<lbrace>\<lambda>s. range_cover ptr sz (objBitsKO val + gbits) n \<and> n \<noteq> 0 \<and> pspace_aligned' s \<and>
-        pspace_distinct' s \<and> ex_cte_cap_to' p s \<and> pspace_no_overlap' ptr sz s\<rbrace>
+        pspace_distinct' s \<and> pspace_bounded' s \<and> ex_cte_cap_to' p s \<and> pspace_no_overlap' ptr sz s\<rbrace>
   createObjects ptr n val gbits \<lbrace>\<lambda>r. ex_cte_cap_to' p\<rbrace>"
   apply (simp add: ex_cte_cap_to'_def createObjects_def)
   apply (rule hoare_lift_Pf2 [where f="irq_node'"])
@@ -4777,13 +5150,14 @@ lemma createObjects_ex_cte_cap_to [wp]:
 lemma createObjects_orig_obj_at3:
   "\<lbrace>\<lambda>s. obj_at' P p s \<and> range_cover ptr sz (objBitsKO val + gbits) n \<and> n \<noteq> 0 \<and>
         pspace_aligned' s \<and>
-        pspace_distinct' s \<and> pspace_no_overlap' ptr sz s\<rbrace>
+        pspace_distinct' s \<and> pspace_bounded' s  \<and> pspace_no_overlap' ptr sz s\<rbrace>
   createObjects ptr n val gbits \<lbrace>\<lambda>r. obj_at' P p\<rbrace>"
   by (wp createObjects_orig_obj_at'[where sz = sz] | simp add: createObjects_def)+
 
 lemma createObjects_sch:
-  "\<lbrace>(\<lambda>s. sch_act_wf (ksSchedulerAction s) s) and pspace_aligned' and pspace_distinct' and pspace_no_overlap' ptr sz
-      and K (range_cover ptr sz (objBitsKO val + gbits) n \<and> n \<noteq> 0)\<rbrace>
+  "\<lbrace>(\<lambda>s. sch_act_wf (ksSchedulerAction s) s) and pspace_aligned' and pspace_distinct'
+    and pspace_bounded' and pspace_no_overlap' ptr sz
+    and K (range_cover ptr sz (objBitsKO val + gbits) n \<and> n \<noteq> 0)\<rbrace>
   createObjects ptr n val gbits
   \<lbrace>\<lambda>rv s. sch_act_wf (ksSchedulerAction s) s\<rbrace>"
   apply (rule hoare_gen_asm)
@@ -4791,21 +5165,19 @@ lemma createObjects_sch:
   done
 
 lemma createObjects_queues:
-  "\<lbrace>\<lambda>s. valid_queues s \<and>  pspace_aligned' s \<and> pspace_distinct' s \<and>
+  "\<lbrace>\<lambda>s. valid_queues s \<and>  pspace_aligned' s \<and> pspace_distinct' s \<and> pspace_bounded' s \<and>
         pspace_no_overlap' ptr sz s \<and> range_cover ptr sz (objBitsKO val + gbits) n \<and> n \<noteq> 0\<rbrace>
   createObjects ptr n val gbits
   \<lbrace>\<lambda>rv. valid_queues\<rbrace>"
   apply (wp valid_queues_lift_asm [unfolded pred_conj_def, OF createObjects_orig_obj_at3]
             createObjects_pred_tcb_at' [unfolded pred_conj_def])
-      apply fastforce
-     apply wp+
   apply fastforce
   done
 
 lemma createObjects_queues':
   assumes no_tcb: "\<And>t. projectKO_opt val \<noteq> Some (t::tcb)"
   shows
-  "\<lbrace>\<lambda>s. valid_queues' s \<and>  pspace_aligned' s \<and> pspace_distinct' s \<and>
+  "\<lbrace>\<lambda>s. valid_queues' s \<and>  pspace_aligned' s \<and> pspace_distinct' s \<and> pspace_bounded' s \<and>
         pspace_no_overlap' ptr sz s \<and> range_cover ptr sz (objBitsKO val + gbits) n \<and> n \<noteq> 0\<rbrace>
   createObjects ptr n val gbits
   \<lbrace>\<lambda>rv. valid_queues'\<rbrace>"
@@ -4817,6 +5189,31 @@ lemma createObjects_queues':
    apply wp
   using no_tcb
   apply fastforce
+  done
+
+lemma createObjects_release_queue:
+  "\<lbrace>\<lambda>s. valid_release_queue s \<and>  pspace_aligned' s \<and> pspace_distinct' s \<and> pspace_bounded' s \<and>
+        pspace_no_overlap' ptr sz s \<and> range_cover ptr sz (objBitsKO val + gbits) n \<and> n \<noteq> 0\<rbrace>
+  createObjects ptr n val gbits
+  \<lbrace>\<lambda>rv. valid_release_queue\<rbrace>"
+  by (wp valid_release_queue_lift_asm [unfolded pred_conj_def, OF createObjects_orig_obj_at3]
+            createObjects_pred_tcb_at' [unfolded pred_conj_def])
+     fastforce
+
+lemma createObjects_release_queue':
+  assumes no_tcb: "\<And>t. projectKO_opt val \<noteq> Some (t::tcb)"
+  shows
+  "\<lbrace>\<lambda>s. valid_release_queue' s \<and>  pspace_aligned' s \<and> pspace_distinct' s \<and> pspace_bounded' s \<and>
+        pspace_no_overlap' ptr sz s \<and> range_cover ptr sz (objBitsKO val + gbits) n \<and> n \<noteq> 0\<rbrace>
+  createObjects ptr n val gbits
+  \<lbrace>\<lambda>rv. valid_release_queue'\<rbrace>"
+  apply (simp add: createObjects_def)
+  apply (wp valid_release_queue_lift_asm')
+    apply (wp createObjects_orig_obj_at2')
+    apply clarsimp
+    apply assumption
+   apply wp
+  apply (fastforce simp: no_tcb simp del: projectKOs split: option.splits)
   done
 
 lemma createObjects_no_cte_ifunsafe':
@@ -4844,7 +5241,7 @@ lemma createObjects_no_cte_ifunsafe':
 lemma createObjects_no_cte_valid_global:
   assumes no_cte: "\<And>c. projectKO_opt val \<noteq> Some (c::cte)"
   assumes no_tcb: "\<And>t. projectKO_opt val \<noteq> Some (t::tcb)"
-  shows "\<lbrace>\<lambda>s. pspace_aligned' s \<and> pspace_distinct' s \<and>
+  shows "\<lbrace>\<lambda>s. pspace_aligned' s \<and> pspace_distinct' s \<and> pspace_bounded' s \<and>
         pspace_no_overlap' ptr sz s \<and>
         range_cover ptr sz (objBitsKO val + gbits) n \<and> n \<noteq> 0 \<and>
         valid_global_refs' s\<rbrace>
@@ -4873,7 +5270,7 @@ lemma createObjects'_typ_at:
   "\<lbrace>\<lambda>s. n \<noteq> 0 \<and>
         range_cover ptr sz (objBitsKO val + gbits) n \<and>
         typ_at' T p s \<and>
-        pspace_aligned' s \<and> pspace_distinct' s \<and>
+        pspace_aligned' s \<and> pspace_distinct' s \<and> pspace_bounded' s \<and>
         pspace_no_overlap' ptr sz s\<rbrace>
   createObjects' ptr n val gbits \<lbrace>\<lambda>r s. typ_at' T p s\<rbrace>"
   apply (rule hoare_grab_asm)+
@@ -4913,7 +5310,7 @@ lemma createObjects'_typ_at:
   done
 
 lemma createObjects_valid_arch:
-  "\<lbrace>\<lambda>s. valid_arch_state' s \<and> pspace_aligned' s \<and> pspace_distinct' s \<and>
+  "\<lbrace>\<lambda>s. valid_arch_state' s \<and> pspace_aligned' s \<and> pspace_distinct' s \<and> pspace_bounded' s \<and>
         pspace_no_overlap' ptr sz s \<and> range_cover ptr sz (objBitsKO val + gbits) n \<and> n \<noteq> 0 \<rbrace>
       createObjects ptr n val gbits
    \<lbrace>\<lambda>rv s. valid_arch_state' s\<rbrace>"
@@ -4929,7 +5326,7 @@ lemma createObjects_valid_arch:
   done
 
 lemma createObjects_irq_state:
-  "\<lbrace>\<lambda>s. pspace_aligned' s \<and> pspace_distinct' s \<and>
+  "\<lbrace>\<lambda>s. pspace_aligned' s \<and> pspace_distinct' s \<and> pspace_bounded' s \<and>
         pspace_no_overlap' ptr sz s \<and>
         range_cover ptr sz (objBitsKO val + gbits) n \<and> n \<noteq> 0 \<and>
         valid_irq_node' (irq_node' s) s\<rbrace>
@@ -4943,7 +5340,7 @@ lemma createObjects_no_cte_irq_handlers:
   assumes no_cte: "\<And>c. projectKO_opt val \<noteq> Some (c::cte)"
   assumes no_tcb: "\<And>t. projectKO_opt val \<noteq> Some (t::tcb)"
   shows
-  "\<lbrace>\<lambda>s. pspace_aligned' s \<and> pspace_distinct' s \<and>
+  "\<lbrace>\<lambda>s. pspace_aligned' s \<and> pspace_distinct' s \<and> pspace_bounded' s \<and>
         pspace_no_overlap' ptr sz s \<and>
         range_cover ptr sz (objBitsKO val + gbits) n \<and> n \<noteq> 0 \<and>
         valid_irq_handlers' s\<rbrace>
@@ -4955,7 +5352,7 @@ lemma createObjects_no_cte_irq_handlers:
   using no_cte no_tcb by (auto simp: split_def split: option.splits)
 
 lemma createObjects_cur':
-  "\<lbrace>\<lambda>s. pspace_aligned' s \<and> pspace_distinct' s \<and>
+  "\<lbrace>\<lambda>s. pspace_aligned' s \<and> pspace_distinct' s \<and> pspace_bounded' s \<and>
         pspace_no_overlap' ptr sz s \<and> range_cover ptr sz (objBitsKO val + gbits) n \<and> n \<noteq> 0 \<and>
         cur_tcb' s\<rbrace>
       createObjects ptr n val gbits
@@ -4969,7 +5366,7 @@ lemma createObjects_cur':
 
 lemma createObjects_vms'[wp]:
   "\<lbrace>(\<lambda>_.  (range_cover ptr sz  (objBitsKO val + gbits) n \<and> 0 < n)) and pspace_aligned' and
-     pspace_distinct' and pspace_no_overlap' ptr sz and valid_machine_state'\<rbrace>
+     pspace_distinct' and pspace_bounded' and pspace_no_overlap' ptr sz and valid_machine_state'\<rbrace>
       createObjects ptr n val gbits
    \<lbrace>\<lambda>rv. valid_machine_state'\<rbrace>"
   apply (simp add: valid_machine_state'_def pointerInUserData_def pointerInDeviceData_def
@@ -5000,7 +5397,7 @@ lemma untyped_zero_ranges_cte_def:
   done
 
 lemma createObjects_untyped_ranges_zero':
-  assumes moKO: "makeObjectKO dev ty = Some val"
+  assumes moKO: "makeObjectKO dev us d ty = Some val"
   shows
   "\<lbrace>ct_active' and valid_pspace' and pspace_no_overlap' ptr sz
        and untyped_ranges_zero'
@@ -5026,9 +5423,13 @@ lemma createObjects_untyped_ranges_zero':
   done
 
 lemma createObjects_no_cte_invs:
-  assumes moKO: "makeObjectKO dev ty = Some val"
+  assumes moKO: "makeObjectKO dev us d ty = Some val"
   assumes no_cte: "\<And>c. projectKO_opt val \<noteq> Some (c::cte)"
   assumes no_tcb: "\<And>t. projectKO_opt val \<noteq> Some (t::tcb)"
+  and     tysc: "ty = Inr (APIObjectType SchedContextObject) \<longrightarrow> sc_size_bounds us"
+  and     mdom: "ty =
+        Inr (APIObjectType ArchTypes_H.apiobject_type.TCBObject) \<longrightarrow>
+        d \<le> maxDomain"
   shows
   "\<lbrace>\<lambda>s. range_cover ptr sz ((objBitsKO val) + gbits) n \<and> n \<noteq> 0
         \<and> sz \<le> maxUntypedSizeBits \<and> canonical_address (ptr && ~~ mask sz)
@@ -5037,37 +5438,22 @@ lemma createObjects_no_cte_invs:
         \<and> pspace_no_overlap' ptr sz s \<and> ptr \<noteq> 0
         \<and> {ptr .. (ptr && ~~ mask sz) + 2 ^ sz - 1} \<inter> kernel_data_refs = {}
         \<and> caps_overlap_reserved' {ptr..ptr + of_nat (n * 2 ^ gbits * 2 ^ objBitsKO val) - 1} s
-        \<and> caps_no_overlap'' ptr sz s \<and> refs_of' val = {} \<and> \<not> live' val\<rbrace>
+        \<and> caps_no_overlap'' ptr sz s \<and> refs_of' val = {} \<and> \<not> live' val
+        \<and> (case val of KOReply r \<Rightarrow> replyNext_of r = None \<and> replyPrev r = None
+                     | _ \<Rightarrow> True)\<rbrace>
   createObjects ptr n val gbits
   \<lbrace>\<lambda>rv. invs'\<rbrace>"
-proof -
-  have co_ct_not_inQ:
-    "\<lbrakk>range_cover ptr sz ((objBitsKO val) + gbits) n; n \<noteq> 0\<rbrakk> \<Longrightarrow>
-     \<lbrace>\<lambda>s. ct_not_inQ s \<and> pspace_no_overlap' ptr sz s \<and> valid_pspace' s\<rbrace>
-      createObjects ptr n val gbits \<lbrace>\<lambda>_. ct_not_inQ\<rbrace>"
-    (is "\<lbrakk> _; _ \<rbrakk> \<Longrightarrow> \<lbrace>\<lambda>s. ct_not_inQ s \<and> ?REST s\<rbrace> _ \<lbrace>_\<rbrace>")
-    apply (simp add: ct_not_inQ_def)
-    apply (rule_tac Q="\<lambda>s. (ksSchedulerAction s = ResumeCurrentThread) \<longrightarrow>
-                             (obj_at' (Not \<circ> tcbQueued) (ksCurThread s) s \<and> ?REST s)"
-             in hoare_pre_imp, clarsimp)
-    apply (rule hoare_convert_imp [OF createObjects_nosch])
-    apply (rule hoare_weaken_pre)
-     apply (wps createObjects_ct)
-     apply (wp createObjects_obj_at_other)
-      apply (simp)+
-    done
-  show ?thesis
   apply (rule hoare_grab_asm)+
-   apply (clarsimp simp: invs'_def valid_state'_def)
-   apply wp
-   apply (rule hoare_pre)
+  apply (clarsimp simp: invs'_def valid_dom_schedule'_def)
+  apply (rule hoare_pre)
    apply (rule hoare_vcg_conj_lift)
-   apply (simp add: createObjects_def,wp createObjects_valid_pspace_untyped')
-   apply (wp assms | simp add: objBits_def)+
+    apply (simp add: createObjects_def,wp createObjects_valid_pspace_untyped')
+           apply (wp assms | simp add: objBits_def)+
    apply (wp createObjects_sch createObjects_queues)
    apply (rule hoare_vcg_conj_lift)
     apply (simp add: createObjects_def)
     apply (wp createObjects_state_refs_of'')
+    apply (wpsimp wp: createObjects_list_refs_of_replies'')
    apply (rule hoare_vcg_conj_lift)
     apply (simp add: createObjects_def)
     apply (wp createObjects_iflive')
@@ -5076,116 +5462,56 @@ proof -
              createObjects_valid_arch createObjects_irq_state
              createObjects_no_cte_irq_handlers createObjects_cur'
              createObjects_queues' [OF no_tcb]
+             createObjects_release_queue' [OF no_tcb]
+             createObjects_release_queue
              assms | simp add: objBits_def )+
-  apply (rule hoare_vcg_conj_lift)
-   apply (simp add: createObjects_def)
-   apply (wp createObjects_idle')
-   apply (wp createObjects_no_cte_ifunsafe' irqs_masked_lift
-             createObjects_idle' createObjects_no_cte_valid_global
-             createObjects_valid_arch createObjects_irq_state
-             createObjects_no_cte_irq_handlers createObjects_cur'
-             createObjects_queues' [OF no_tcb] assms
-             createObjects_pspace_domain_valid co_ct_not_inQ
-             createObjects_ct_idle_or_in_cur_domain'
-             createObjects_untyped_ranges_zero'[OF moKO]
-         | simp)+
+   apply (rule hoare_vcg_conj_lift)
+    apply (wp createObjects_no_cte_ifunsafe' irqs_masked_lift
+              createObjects_idle' createObjects_no_cte_valid_global
+              createObjects_valid_arch createObjects_irq_state
+              createObjects_no_cte_irq_handlers createObjects_cur'
+              createObjects_queues' [OF no_tcb] assms
+              createObjects_release_queue' [OF no_tcb]
+              createObjects_release_queue
+              createObjects_pspace_domain_valid
+              createObjects_ct_idle_or_in_cur_domain'
+              createObjects_untyped_ranges_zero'[OF moKO]
+          | simp)+
   apply clarsimp
-  using no_cte no_tcb
   apply ((intro conjI; assumption?); simp add: valid_pspace'_def objBits_def)
-  apply (fastforce simp add: split_def split: option.splits)
-  apply (clarsimp simp: invs'_def no_tcb valid_state'_def no_cte  split: option.splits)
   done
-qed
 
 lemma corres_retype_update_gsI:
   assumes not_zero: "n \<noteq> 0"
   and      aligned: "is_aligned ptr (objBitsKO ko + gbits)"
-  and obj_bits_api: "obj_bits_api (APIType_map2 ty) us =
-                     objBitsKO ko + gbits"
-  and        check: "sz < obj_bits_api (APIType_map2 ty) us \<longleftrightarrow>
-                     sz < objBitsKO ko + gbits"
-  and          usv: "APIType_map2 ty = Structures_A.CapTableObject \<Longrightarrow> 0 < us"
-  and           ko: "makeObjectKO dev ty = Some ko"
+  and obj_bits_api: "obj_bits_api (APIType_map2 ty) us = objBitsKO ko + gbits"
+  and        check: "sz < obj_bits_api (APIType_map2 ty) us \<longleftrightarrow> sz < objBitsKO ko + gbits"
+  and           ko: "makeObjectKO dev us d ty = Some ko"
+  and            tysc: "ty = Inr (APIObjectType SchedContextObject) \<longrightarrow> min_sched_context_bits \<le> us"
   and          orr: "obj_bits_api (APIType_map2 ty) us \<le> sz \<Longrightarrow>
-                     obj_relation_retype
-                       (default_object (APIType_map2 ty) dev us) ko"
+                     obj_relation_retype (default_object (APIType_map2 ty) dev us d) ko"
   and        cover: "range_cover ptr sz (obj_bits_api (APIType_map2 ty) us) n"
   and            f: "f = update_gs (APIType_map2 ty) us"
   shows "corres (\<lambda>rv rv'. rv' = g rv)
          (\<lambda>s. valid_pspace s \<and> pspace_no_overlap_range_cover ptr sz s
-            \<and> valid_mdb s \<and> valid_etcbs s \<and> valid_list s)
+            \<and> valid_mdb s \<and> valid_list s)
          (\<lambda>s. pspace_aligned' s \<and> pspace_distinct' s \<and>
-              pspace_no_overlap' ptr sz s)
-         (retype_region2 ptr n us (APIType_map2 ty) dev)
+              pspace_no_overlap' ptr sz s \<and>
+              (ty = Inr (APIObjectType TCBObject) \<longrightarrow> d = ksCurDomain s))
+         (retype_region ptr n us (APIType_map2 ty) dev)
          (do addrs \<leftarrow> createObjects ptr n ko gbits;
              _ \<leftarrow> modify (f (set addrs));
              return (g addrs)
           od)"
-  using corres_retype' [OF not_zero aligned obj_bits_api check usv ko orr cover]
-  by (simp add: f)
+  using corres_retype' [OF not_zero aligned obj_bits_api check ko tysc orr cover]
+  by (clarsimp simp: f)
 
-lemma gcd_corres: "corres (=) \<top> \<top> (gets cur_domain) curDomain"
+lemma gcd_corres[corres]: "corres (=) \<top> \<top> (gets cur_domain) curDomain"
   by (simp add: curDomain_def state_relation_def)
-
-lemma retype_region2_extra_ext_mapM_x_corres:
-  shows "corres dc
-           (valid_etcbs and (\<lambda>s. \<forall>addr\<in>set addrs. tcb_at addr s))
-           (\<lambda>s. \<forall>addr\<in>set addrs. tcb_at' addr s)
-           (retype_region2_extra_ext addrs Structures_A.apiobject_type.TCBObject)
-           (mapM_x (\<lambda>addr. do cdom \<leftarrow> curDomain;
-                              threadSet (tcbDomain_update (\<lambda>_. cdom)) addr
-                           od)
-             addrs)"
-  apply (rule corres_guard_imp)
-    apply (simp add: retype_region2_extra_ext_def curDomain_mapM_x_futz[symmetric] when_def)
-    apply (rule corres_split_eqr[OF _ gcd_corres])
-      apply (rule_tac S="Id \<inter> {(x, y). x \<in> set addrs}"
-                  and P="\<lambda>s. (\<forall>t \<in> set addrs. tcb_at t s) \<and> valid_etcbs s"
-                  and P'="\<lambda>s. \<forall>t \<in> set addrs. tcb_at' t s"
-                   in corres_mapM_x)
-          apply simp
-          apply (rule corres_guard_imp)
-            apply (rule ethread_set_corres, simp_all add: etcb_relation_def non_exst_same_def)[1]
-            apply (case_tac tcb')
-            apply simp
-           apply fastforce
-          apply fastforce
-         apply (wp hoare_vcg_ball_lift | simp)+
-      apply auto[1]
-     apply (wp | simp add: curDomain_def)+
-  done
-
-lemma retype_region2_extra_ext_trivial:
-  "ty \<noteq> APIType_map2 (Inr (APIObjectType apiobject_type.TCBObject))
-      \<Longrightarrow> retype_region2_extra_ext ptrs ty = return ()"
-by (simp add: retype_region2_extra_ext_def when_def APIType_map2_def)
-
-lemma retype_region2_retype_region_PageTableObject:
-  "retype_region ptr n us (APIType_map2 (Inr PageTableObject)) dev =
-  (retype_region2 ptr n us (APIType_map2 (Inr PageTableObject)) dev :: obj_ref list det_ext_monad)"
-  by (simp add: retype_region2_ext_retype_region retype_region2_extra_ext_def when_def
-                APIType_map2_def)
-
-lemma retype_region2_valid_etcbs[wp]:"\<lbrace>valid_etcbs\<rbrace> retype_region2 a b c d dev \<lbrace>\<lambda>_. valid_etcbs\<rbrace>"
-  apply (simp add: retype_region2_def)
-  apply (simp add: retype_region2_ext_def bind_assoc)
-  apply wp
-  apply (clarsimp simp del: fun_upd_apply)
-  apply (blast intro: valid_etcb_fold_update)
-  done
-
-lemma retype_region2_obj_at:
-  assumes tytcb: "ty = Structures_A.apiobject_type.TCBObject"
-  shows "\<lbrace>\<top>\<rbrace> retype_region2 ptr n us ty dev \<lbrace>\<lambda>rv s. \<forall>x \<in> set rv. tcb_at x s\<rbrace>"
-  using tytcb unfolding retype_region2_def
-  apply (simp only: return_bind bind_return foldr_upd_app_if fun_app_def K_bind_def)
-  apply (wp dxo_wp_weak | simp)+
-  apply (auto simp: obj_at_def default_object_def is_tcb_def)
-  done
 
 lemma createObjects_tcb_at':
   "\<lbrakk>range_cover ptr sz (objBitsKO (injectKOS (makeObject::tcb))) n; n \<noteq> 0\<rbrakk> \<Longrightarrow>
-   \<lbrace>\<lambda>s. pspace_no_overlap' ptr sz s \<and> pspace_aligned' s \<and> pspace_distinct' s\<rbrace>
+   \<lbrace>\<lambda>s. pspace_no_overlap' ptr sz s \<and> pspace_aligned' s \<and> pspace_distinct' s \<and> pspace_bounded' s\<rbrace>
    createObjects ptr n (KOTCB makeObject) 0 \<lbrace>\<lambda>ptrs s. \<forall>addr\<in>set ptrs. tcb_at' addr s\<rbrace>"
   apply (rule hoare_strengthen_post[OF createObjects_ko_at_strg[where val = "(makeObject :: tcb)"]])
   apply (auto simp: obj_at'_def project_inject objBitsKO_def objBits_def makeObject_tcb)
@@ -5207,11 +5533,13 @@ lemma data_page_relation_retype:
 lemma corres_retype_region_createNewCaps:
   "corres ((\<lambda>r r'. length r = length r' \<and> list_all2 cap_relation r r')
                \<circ> map (\<lambda>ref. default_cap (APIType_map2 (Inr ty)) ref us dev))
-            (\<lambda>s. valid_pspace s \<and> valid_mdb s \<and> valid_etcbs s \<and> valid_list s \<and> valid_arch_state s
+            (\<lambda>s. valid_pspace s \<and> valid_mdb s \<and> valid_list s \<and> valid_arch_state s
                    \<and> caps_no_overlap y sz s \<and> pspace_no_overlap_range_cover y sz s
                    \<and> caps_overlap_reserved {y..y + of_nat n * 2 ^ (obj_bits_api (APIType_map2 (Inr ty)) us) - 1} s
                    \<and> (\<exists>slot. cte_wp_at (\<lambda>c. up_aligned_area y sz \<subseteq> cap_range c \<and> cap_is_device c = dev) slot s)
-                   \<and> (APIType_map2 (Inr ty) = Structures_A.CapTableObject \<longrightarrow> 0 < us))
+                   \<and> (APIType_map2 (Inr ty) = Structures_A.CapTableObject \<longrightarrow> 0 < us)
+                   \<and> (APIType_map2 (Inr ty) = Structures_A.SchedContextObject
+                            \<longrightarrow> sc_size_bounds us))
             (\<lambda>s. pspace_aligned' s \<and> pspace_distinct' s \<and> pspace_no_overlap' y sz s
                   \<and> valid_pspace' s \<and> valid_arch_state' s
                   \<and> range_cover y sz (obj_bits_api (APIType_map2 (Inr ty)) us) n \<and> n\<noteq> 0)
@@ -5220,160 +5548,170 @@ lemma corres_retype_region_createNewCaps:
                 return x od)
             (createNewCaps ty y n us dev)"
   including no_take_bit
-  apply (rule_tac F="range_cover y sz (obj_bits_api (APIType_map2 (Inr ty)) us) n
-                      \<and> n \<noteq> 0 \<and> (APIType_map2 (Inr ty) = Structures_A.CapTableObject \<longrightarrow> 0 < us)"
-           in corres_req, simp)
-  apply (clarsimp simp add: createNewCaps_def toAPIType_def split del: if_split cong: if_cong)
+  apply (rule_tac F="range_cover y sz
+                       (obj_bits_api (APIType_map2 (Inr ty)) us) n \<and>
+                     n \<noteq> 0 \<and>
+                     (APIType_map2 (Inr ty) = Structures_A.CapTableObject
+                       \<longrightarrow> 0 < us)
+                     \<and> (APIType_map2 (Inr ty) = Structures_A.SchedContextObject
+                            \<longrightarrow> sc_size_bounds us)"
+            in corres_req, simp)
+  apply (clarsimp simp add: createNewCaps_def toAPIType_def
+                 split del: if_split cong: if_cong)
   apply (subst init_arch_objects_APIType_map2)
-  apply (cases ty, simp_all add: Arch_createNewCaps_def split del: if_split)
+  apply (cases ty, simp_all add: Arch_createNewCaps_def
+                      split del: if_split)
       apply (rename_tac apiobject_type)
       apply (case_tac apiobject_type, simp_all split del: if_split)
-          \<comment> \<open>Untyped\<close>
-          apply (simp add: retype_region_def obj_bits_api_def APIType_map2_def
-                      split del: if_split cong: if_cong)
-          apply (subst upto_enum_red')
-           apply (drule range_cover_not_zero[rotated])
-            apply simp
-           apply unat_arith
-          apply (clarsimp simp: list_all2_same enum_word_def range_cover.unat_of_nat_n
-                                list_all2_map1 list_all2_map2 ptr_add_def fromIntegral_def
-                                toInteger_nat fromInteger_nat)
-          apply (subst unat_of_nat_minus_1)
-            apply (rule le_less_trans[OF range_cover.range_cover_n_le(2) power_strict_increasing])
+            \<comment> \<open>Untyped\<close>
+            apply (simp     add: retype_region_def obj_bits_api_def
+                                 APIType_map2_def
+                      split del: if_split
+                           cong: if_cong)
+            apply (subst upto_enum_red')
+             apply (drule range_cover_not_zero[rotated])
               apply simp
-             apply (clarsimp simp: range_cover_def)
-             apply (arith+)[4]
-         \<comment> \<open>TCB, EP, NTFN\<close>
-         apply (simp_all add: retype_region2_ext_retype_region
-                              bind_cong[OF curDomain_mapM_x_futz refl, unfolded bind_assoc]
-                         split del: if_split)[8]
-         apply (rule corres_guard_imp)
-           apply (rule corres_split_eqr)
-              apply (rule corres_split_nor)
-                 apply (rule corres_trivial, simp)
-                 apply (clarsimp simp: list_all2_same list_all2_map1 list_all2_map2
-                                       objBits_simps APIType_map2_def)
-                apply (simp add: APIType_map2_def)
-                apply (rule retype_region2_extra_ext_mapM_x_corres)
-               apply wp
-              apply wp
-             apply (rule corres_retype[where 'a = tcb],
-                    simp_all add: obj_bits_api_def objBits_simps' pageBits_def
-                                  APIType_map2_def makeObjectKO_def
-                                  other_objs_default_relation)[1]
-             apply (fastforce simp: range_cover_def)
-            apply ((wp retype_region2_obj_at | simp add: APIType_map2_def)+)[1]
-           apply ((wp createObjects_tcb_at'[where sz=sz]
-                   | simp add: APIType_map2_def objBits_simps' obj_bits_api_def)+)[1]
+             apply unat_arith
+            apply (clarsimp simp: list_all2_same enum_word_def  range_cover.unat_of_nat_n
+                                  list_all2_map1 list_all2_map2
+                                  ptr_add_def fromIntegral_def toInteger_nat fromInteger_nat)
+            apply (subst unat_of_nat_minus_1)
+              apply (rule le_less_trans[OF range_cover.range_cover_n_le(2) power_strict_increasing])
+                apply simp
+               apply (clarsimp simp: range_cover_def)
+               apply (arith+)[4]
+           \<comment> \<open>TCB\<close>
+             apply (simp_all add: curDomain_def split del: if_split)
+             apply (rule corres_underlying_gets_pre_rhs[rotated])
+              apply (rule gets_sp)
+             apply (rule corres_guard_imp)
+               apply (rule corres_bind_return)
+               apply (rule corres_split_eqr)
+                  apply (rule corres_returnTT, simp)
+                  apply (clarsimp simp: list_all2_same list_all2_map1 list_all2_map2
+                                        objBits_simps APIType_map2_def)
+                 apply (rule corres_retype[where 'a = tcb],
+                        simp_all add: obj_bits_api_def objBits_simps' pageBits_def
+                                      APIType_map2_def makeObjectKO_def)[1]
+                  apply (fastforce simp: range_cover_def)
+                 apply (simp add: other_objs_default_relation)
+                apply ((wp | simp add: APIType_map2_def)+)[1]
+               apply ((wp createObjects_tcb_at'[where sz=sz] | simp add: APIType_map2_def objBits_simps' obj_bits_api_def)+)[1]
+              apply simp
+             apply simp
+          \<comment> \<open>CapTable\<close>
+          apply (find_goal \<open>match premises in "_ = ArchTypes_H.apiobject_type.CapTableObject" \<Rightarrow> \<open>-\<close>\<close>)
+          apply (subst bind_assoc_reverse[of "createObjects y n (KOCTE makeObject) us"])
+          apply (subst liftM_def [of "map (\<lambda>addr. capability.CNodeCap addr us 0 0)", symmetric])
           apply simp
-         apply simp
-        apply (subst retype_region2_extra_ext_trivial)
-         apply (simp add: APIType_map2_def)
+          apply (rule corres_rel_imp)
+           apply (rule corres_guard_imp)
+             apply (rule corres_retype_update_gsI,
+                    simp_all add: obj_bits_api_def objBits_simps' pageBits_def
+                                  APIType_map2_def makeObjectKO_def slot_bits_def
+                                  field_simps ext)[1]
+              apply ((clarsimp simp : range_cover_def APIType_map2_def word_bits_def
+                                       list_all2_same list_all2_map1 list_all2_map2
+                     | rule captable_relation_retype)+)[5]
+         \<comment> \<open>EP, NTFN\<close>
+         apply (simp add: liftM_def[symmetric] split del: if_split)
+         apply (rule corres_rel_imp)
+          apply (rule corres_guard_imp)
+            apply (rule corres_retype[where 'a = endpoint],
+                   simp_all add: obj_bits_api_def objBits_simps' pageBits_def
+                                 APIType_map2_def makeObjectKO_def
+                                 other_objs_default_relation)[1]
+            apply ((simp add: range_cover_def APIType_map2_def
+                              list_all2_same list_all2_map1 list_all2_map2)+)[4]
         apply (simp add: liftM_def[symmetric] split del: if_split)
         apply (rule corres_rel_imp)
          apply (rule corres_guard_imp)
-           apply (rule corres_retype[where 'a = endpoint],
-                  simp_all add: obj_bits_api_def objBits_simps' pageBits_def APIType_map2_def
-                                makeObjectKO_def other_objs_default_relation)[1]
-           apply (fastforce simp: range_cover_def)
-          apply simp
-         apply simp
-        apply (clarsimp simp: list_all2_same list_all2_map1 list_all2_map2 objBits_simps
-                              APIType_map2_def)
-       apply (subst retype_region2_extra_ext_trivial)
-        apply (simp add: APIType_map2_def)
+         apply (rule corres_retype[where 'a = notification],
+                simp_all add: obj_bits_api_def objBits_simps' pageBits_def
+                              APIType_map2_def makeObjectKO_def
+                              other_objs_default_relation)[1]
+           apply ((simp add: range_cover_def APIType_map2_def
+                             list_all2_same list_all2_map1 list_all2_map2)+)[4]
+       \<comment> \<open>SchedContext\<close>
        apply (simp add: liftM_def[symmetric] split del: if_split)
        apply (rule corres_rel_imp)
         apply (rule corres_guard_imp)
-          apply (rule corres_retype[where 'a = notification],
-                 simp_all add: obj_bits_api_def objBits_simps' pageBits_def APIType_map2_def
-                               makeObjectKO_def other_objs_default_relation)[1]
-          apply (fastforce simp: range_cover_def)
-         apply simp
-        apply simp
-       apply (clarsimp simp: list_all2_same list_all2_map1 list_all2_map2 objBits_simps
-                             APIType_map2_def)
-      \<comment> \<open>CapTable\<close>
-      apply (subst retype_region2_extra_ext_trivial)
-       apply (simp add: APIType_map2_def)
-      apply (subst bind_assoc_reverse[of "createObjects y n (KOCTE makeObject) us"])
-      apply (subst liftM_def[of "map (\<lambda>addr. capability.CNodeCap addr us 0 0)", symmetric])
-      apply simp
+          apply (rule corres_retype[where 'a = sched_context],
+                 simp_all add: obj_bits_api_def objBits_simps' pageBits_def
+                               APIType_map2_def makeObjectKO_def scBits_simps
+                               sc_relation_retype)[1]
+          apply ((simp add: range_cover_def APIType_map2_def sc_size_bounds_def
+                            list_all2_same list_all2_map1 list_all2_map2 sc_const_eq)+)[4]
+      \<comment> \<open>Reply\<close>
+      apply (simp add: liftM_def[symmetric] split del: if_split)
       apply (rule corres_rel_imp)
        apply (rule corres_guard_imp)
-         apply (rule corres_retype_update_gsI,
-                simp_all add: obj_bits_api_def objBits_simps' pageBits_def APIType_map2_def
-                              makeObjectKO_def slot_bits_def field_simps ext)[1]
-          apply (simp add: range_cover_def)
-         apply (rule captable_relation_retype,simp add: range_cover_def word_bits_def)
-        apply simp
-       apply simp
-      apply (clarsimp simp: list_all2_same list_all2_map1 list_all2_map2 objBits_simps
-                            allRights_def APIType_map2_def
-                      split del: if_split)
-     apply (in_case \<open>HugePageObject\<close>)
-     apply (subst retype_region2_extra_ext_trivial)
-      apply (simp add: APIType_map2_def)
+         apply (rule corres_retype[where 'a = reply],
+                simp_all add: obj_bits_api_def objBits_simps' pageBits_def
+                              APIType_map2_def makeObjectKO_def
+                              reply_relation_retype)[1]
+         apply ((simp add: range_cover_def APIType_map2_def
+                           list_all2_same list_all2_map1 list_all2_map2)+)[4]
+     \<comment> \<open>HugePageObject\<close>
      apply (simp add: corres_liftM2_simp[unfolded liftM_def] split del: if_split)
      apply (rule corres_rel_imp)
       apply (simp add: init_arch_objects_APIType_map2_noop split del: if_split)
       apply (rule corres_guard_imp)
-        apply (rule corres_retype_update_gsI;
-               clarsimp simp: obj_bits_api_def3 APIType_map2_def objBits_simps ext
-                              default_object_def default_arch_object_def makeObjectKO_def
-                              data_page_relation_retype bit_simps
-                       elim!: range_cover.aligned;
-               assumption)
-       apply fastforce+
-   apply (simp add: APIType_map2_def arch_default_cap_def vm_read_write_def vmrights_map_def
-                    list_all2_map1 list_all2_map2 list_all2_same)
-    apply (in_case \<open>SmallPageObject\<close>)
-    apply (subst retype_region2_extra_ext_trivial)
-     apply (simp add: APIType_map2_def)
+        apply (rule corres_retype_update_gsI,
+               simp_all add: APIType_map2_def makeObjectKO_def
+                   arch_default_cap_def obj_bits_api_def
+                   default_object_def default_arch_object_def pageBits_def
+                   ext objBits_simps range_cover.aligned,
+                   simp_all add: data_page_relation_retype)[1]
+       apply simp+
+     apply (simp add: APIType_map2_def arch_default_cap_def vmrights_map_def
+                      vm_read_write_def list_all2_map1 list_all2_map2 list_all2_same)
+    \<comment> \<open>SmallPageObject\<close>
     apply (simp add: corres_liftM2_simp[unfolded liftM_def] split del: if_split)
     apply (rule corres_rel_imp)
      apply (simp add: init_arch_objects_APIType_map2_noop split del: if_split)
      apply (rule corres_guard_imp)
-       apply (rule corres_retype_update_gsI;
-              clarsimp simp: obj_bits_api_def3 APIType_map2_def objBits_simps ext
-                             default_object_def default_arch_object_def makeObjectKO_def
-                             data_page_relation_retype
-                      elim!: range_cover.aligned;
-              assumption)
-      apply fastforce+
-     apply (simp add: APIType_map2_def arch_default_cap_def vm_read_write_def vmrights_map_def
-                      list_all2_map1 list_all2_map2 list_all2_same)
-   apply (in_case \<open>LargePageObject\<close>)
-   apply (subst retype_region2_extra_ext_trivial)
-    apply (simp add: APIType_map2_def)
+       apply (rule corres_retype_update_gsI,
+              simp_all add: APIType_map2_def makeObjectKO_def
+                            arch_default_cap_def obj_bits_api_def
+                            default_object_def default_arch_object_def pageBits_def
+                            ext objBits_simps range_cover.aligned,
+              simp_all add: data_page_relation_retype)[1]
+      apply simp+
+    apply (simp add: APIType_map2_def arch_default_cap_def vmrights_map_def
+                     vm_read_write_def list_all2_map1 list_all2_map2 list_all2_same)
+   \<comment> \<open>LargePageObject\<close>
    apply (simp add: corres_liftM2_simp[unfolded liftM_def] split del: if_split)
    apply (rule corres_rel_imp)
     apply (simp add: init_arch_objects_APIType_map2_noop split del: if_split)
     apply (rule corres_guard_imp)
-      apply (rule corres_retype_update_gsI;
-             clarsimp simp: obj_bits_api_def3 APIType_map2_def objBits_simps ext
-                            default_object_def default_arch_object_def makeObjectKO_def
-                            data_page_relation_retype
-                     elim!: range_cover.aligned;
-             assumption)
-     apply fastforce+
-    apply (simp add: APIType_map2_def arch_default_cap_def vm_read_write_def vmrights_map_def
-                     list_all2_map1 list_all2_map2 list_all2_same)
-  apply (in_case \<open>PageTableObject\<close>)
-  apply (subst retype_region2_extra_ext_trivial)
-   apply (simp add: APIType_map2_def)
-  apply (simp_all add: corres_liftM2_simp[unfolded liftM_def])
-  apply (rule corres_guard_imp)
+      apply (rule corres_retype_update_gsI,
+             simp_all add: APIType_map2_def makeObjectKO_def
+                           arch_default_cap_def obj_bits_api_def
+                           default_object_def default_arch_object_def pageBits_def
+                           ext objBits_simps range_cover.aligned,
+             simp_all add: data_page_relation_retype)[1]
+     apply simp+
+   apply (simp add: APIType_map2_def arch_default_cap_def vmrights_map_def
+                    vm_read_write_def list_all2_map1 list_all2_map2 list_all2_same)
+  \<comment> \<open>PageTableObject\<close>
+   apply (simp_all add: corres_liftM2_simp[unfolded liftM_def])
+   apply (rule corres_guard_imp)
     apply (simp add: init_arch_objects_APIType_map2_noop)
     apply (rule corres_rel_imp)
-     apply (rule corres_retype[where 'a=pte];
-            simp add: APIType_map2_def obj_bits_api_def default_arch_object_def objBits_simps
-                      bit_simps makeObjectKO_def range_cover.aligned)
+       apply (rule corres_retype[where 'a =pte],
+            simp_all add: APIType_map2_def obj_bits_api_def
+                          default_arch_object_def objBits_simps
+                          ptBits_def pageBits_def pteBits_def
+                          makeObjectKO_def range_cover.aligned
+                          pte_bits_def pt_bits_def word_size_bits_def table_size_def
+                          ptTranslationBits_def)[1]
      apply (rule pagetable_relation_retype)
     apply (wp | simp)+
     apply (clarsimp simp: list_all2_map1 list_all2_map2 list_all2_same
+
                           APIType_map2_def arch_default_cap_def)
-   apply fastforce+
+   apply simp+
   done
 
 end
